Upgrade concurrent/inf_chaselev_deque.

theories/concurrent/inf_chaselev_deque.v
@@ -14,48 +14,88 @@ From caml5.base_logic Require Import
   lib.auth_nat_max
   lib.mono_list.
 From caml5.lang Require Import
+  wise_prophet
+  identifier
   notations
   proofmode.
 From caml5.std Require Import
   inf_array.
 From caml5.concurrent Require Export
   base.
+From caml5.concurrent Require Import
+  ws_deque.
+
+#[local] Program Definition inf_chaselev_deque_prophet := {|
+  typed_prophet_type :=
+    nat * bool * nat * identifier ;
+  typed_prophet_of_val w v :=
+    match w with
+    | (LitV (LitInt front), LitV (LitBool b))%V =>
+        match v with
+        | (LitV (LitInt front'), LitV (LitProphecy id))%V =>
+            Some (Z.to_nat front, b, Z.to_nat front', id)
+        | _ =>
+            None
+        end
+    | _ =>
+        None
+    end ;
+  typed_prophet_to_val '(front, b, front', id) :=
+    ((#front, #b)%V, (#front', #id)%V) ;
+|}.
+Solve Obligations of inf_chaselev_deque_prophet with
+  try done.
+Next Obligation.
+  intros (((front & b) & front') & id) w v ?. simplify. rewrite !Nat2Z.id //.
+Qed.
 
 Class InfChaselevDequeG Σ `{!heapGS Σ} (array : inf_array Σ false) := {
-  inf_chaselev_deque_G_ctl_G : AuthExclG Σ (prodO ZO (nat -d> valO)) ;
+  inf_chaselev_deque_G_ctl_G : AuthExclG Σ (ZO * (nat -d> valO)) ;
   inf_chaselev_deque_G_front_G : AuthNatMaxG Σ ;
   inf_chaselev_deque_G_hist_G : MonoListG Σ val ;
   inf_chaselev_deque_G_pub_G : AuthExclG Σ (listO valO) ;
   inf_chaselev_deque_G_lock_G : ExclG Σ unitO ;
+  inf_chaselev_deque_G_prophet_G : WiseProphetG Σ inf_chaselev_deque_prophet ;
+  inf_chaselev_deque_G_winner_G : AuthExclG Σ (natO * (valO -d> ▶ ∙)) ;
 }.
 #[local] Existing Instance inf_chaselev_deque_G_ctl_G.
 #[local] Existing Instance inf_chaselev_deque_G_front_G.
 #[local] Existing Instance inf_chaselev_deque_G_hist_G.
 #[local] Existing Instance inf_chaselev_deque_G_pub_G.
 #[local] Existing Instance inf_chaselev_deque_G_lock_G.
+#[local] Existing Instance inf_chaselev_deque_G_prophet_G.
+#[local] Existing Instance inf_chaselev_deque_G_winner_G.
 
 Definition inf_chaselev_deque_Σ := #[
-  auth_excl_Σ (prodO ZO (nat -d> valO)) ;
+  auth_excl_Σ (ZO * (nat -d> valO)) ;
   auth_nat_max_Σ ;
   mono_list_Σ val ;
   auth_excl_Σ (listO valO) ;
-  excl_Σ unitO
+  excl_Σ unitO ;
+  wise_prophet_Σ inf_chaselev_deque_prophet ;
+  auth_excl_Σ (natO * (valO -d> ▶ ∙))
 ].
 Lemma subG_inf_chaselev_deque_Σ Σ `{!heapGS Σ} array :
   subG inf_chaselev_deque_Σ Σ →
   InfChaselevDequeG Σ array.
 Proof.
+  pose subG_wise_prophet_Σ.
   solve_inG.
 Qed.
 
+Module base.
 Section inf_chaselev_deque_G.
   Context `{!heapGS Σ} {array} `{inf_chaselev_deque_G : !InfChaselevDequeG Σ array}.
   Implicit Types front : nat.
   Implicit Types back : Z.
   Implicit Types l : loc.
+  Implicit Types p : proph_id.
+  Implicit Types id : identifier.
   Implicit Types v t data : val.
   Implicit Types hist pub : list val.
   Implicit Types priv : nat → val.
+  Implicit Types prophs : list inf_chaselev_deque_prophet.(typed_prophet_type).
+  Implicit Types Φ : val → iProp Σ.
 
   Notation "t '.(front)'" := t.(0)%stdpp
   ( at level 5
@@ -64,6 +104,9 @@ Section inf_chaselev_deque_G.
   ( at level 5
   ) : stdpp_scope.
   Notation "t '.(data)'" := t.(2)%stdpp
+  ( at level 5
+  ) : stdpp_scope.
+  Notation "t '.(prophecy)'" := t.(3)%stdpp
   ( at level 5
   ) : stdpp_scope.
   Notation "t '.(front)'" := t.(0)%E
@@ -75,28 +118,31 @@ Section inf_chaselev_deque_G.
   Notation "t '.(data)'" := t.(2)%E
   ( at level 5
   ) : expr_scope.
+  Notation "t '.(prophecy)'" := t.(3)%E
+  ( at level 5
+  ) : expr_scope.
 
   Definition inf_chaselev_deque_make : val :=
     λ: <>,
-      let: "t" := AllocN #3 #0 in
+      let: "t" := AllocN #4 #0 in
       "t".(data) <- array.(inf_array_make) #() ;;
+      "t".(prophecy) <- NewProph ;;
       "t".
 
   Definition inf_chaselev_deque_push : val :=
     λ: "t" "v",
       let: "back" := !"t".(back) in
-      let: "data" := !"t".(data) in
-      array.(inf_array_set) "data" "back" "v" ;;
+      array.(inf_array_set) !"t".(data) "back" "v" ;;
       "t".(back) <- "back" + #1.
 
   Definition inf_chaselev_deque_steal : val :=
     rec: "inf_chaselev_deque_steal" "t" :=
+      let: "id" := NewId in
       let: "front" := !"t".(front) in
       let: "back" := !"t".(back) in
-      let: "data" := !"t".(data) in
       if: "front" < "back" then (
-        let: "v" := array.(inf_array_get) "data" "front" in
-        if: CAS "t".(front) "front" ("front" + #1) then (
+        let: "v" := array.(inf_array_get) !"t".(data) "front" in
+        if: Snd $ Resolve (CmpXchg "t".(front) "front" ("front" + #1)) !"t".(prophecy) ("front", "id") then (
           SOME "v"
         ) else (
           "inf_chaselev_deque_steal" "t"
@@ -107,21 +153,20 @@ Section inf_chaselev_deque_G.
 
   Definition inf_chaselev_deque_pop : val :=
     λ: "t",
+      let: "id" := NewId in
       let: "back" := !"t".(back) - #1 in
-      let: "data" := !"t".(data) in
       "t".(back) <- "back" ;;
       let: "front" := !"t".(front) in
       if: "back" < "front" then (
         "t".(back) <- "front" ;;
         NONE
       ) else (
-        let: "v" := array.(inf_array_get) "data" "back" in
         if: "front" < "back" then (
-          SOME "v"
+          SOME (array.(inf_array_get) !"t".(data) "back")
         ) else (
-          if: CAS "t".(front) "front" ("front" + #1) then (
+          if: Snd $ Resolve (CmpXchg "t".(front) "front" ("front" + #1)) !"t".(prophecy) ("front", "id") then (
             "t".(back) <- "front" + #1 ;;
-            SOME "v"
+            SOME (array.(inf_array_get) !"t".(data) "back")
           ) else (
             "t".(back) <- "front" + #1 ;;
             NONE
@@ -129,11 +174,20 @@ Section inf_chaselev_deque_G.
         )
       ).
 
-  Notation inf_chaselev_deque_meta_ctl := (nroot .@ "ctl").
-  Notation inf_chaselev_deque_meta_front := (nroot .@ "front").
-  Notation inf_chaselev_deque_meta_hist := (nroot .@ "hist").
-  Notation inf_chaselev_deque_meta_pub := (nroot .@ "pub").
-  Notation inf_chaselev_deque_meta_lock := (nroot .@ "lock").
+  Notation inf_chaselev_deque_meta_ctl :=
+    (nroot .@ "ctl").
+  Notation inf_chaselev_deque_meta_front :=
+    (nroot .@ "front").
+  Notation inf_chaselev_deque_meta_hist :=
+    (nroot .@ "hist").
+  Notation inf_chaselev_deque_meta_pub :=
+    (nroot .@ "pub").
+  Notation inf_chaselev_deque_meta_lock :=
+    (nroot .@ "lock").
+  Notation inf_chaselev_deque_meta_prophet :=
+    (nroot .@ "prophet").
+  Notation inf_chaselev_deque_meta_winner :=
+    (nroot .@ "winner").
 
   #[local] Definition inf_chaselev_deque_ctl₁ γ_ctl back priv :=
     auth_excl_auth (auth_excl_G := inf_chaselev_deque_G_ctl_G) γ_ctl (DfracOwn 1) (back, priv).
@@ -145,12 +199,8 @@ Section inf_chaselev_deque_G.
   #[local] Definition inf_chaselev_deque_front_frag γ_front front :=
     auth_nat_max_frag γ_front front.
 
-  #[local] Definition inf_chaselev_deque_hist_auth γ_hist hist pub :=
-    mono_list_auth γ_hist 1
-      match pub with
-      | [] => hist
-      | v :: _ => hist ++ [v]
-      end.
+  #[local] Definition inf_chaselev_deque_hist_auth γ_hist hist :=
+    mono_list_auth γ_hist 1 hist.
   #[local] Definition inf_chaselev_deque_hist_frag γ_hist i v :=
     mono_list_mapsto γ_hist i v.
 
@@ -162,56 +212,14 @@ Section inf_chaselev_deque_G.
   #[local] Definition inf_chaselev_deque_lock γ_lock :=
     excl γ_lock ().
 
-  #[local] Definition inf_chaselev_deque_state₁ front back pub : iProp Σ :=
-    ⌜(front ≤ back)%Z ∧ length pub = Z.to_nat (back - front)⌝.
-  #[local] Definition inf_chaselev_deque_state₂₁ front back pub : iProp Σ :=
-    ⌜back = front ∧ length pub = 1⌝.
-  #[local] Definition inf_chaselev_deque_state₂₂ front back pub : iProp Σ :=
-    ⌜Z.of_nat front = (back + 1)%Z ∧ pub = []⌝.
-  #[local] Definition inf_chaselev_deque_state₂ γ_lock front back pub : iProp Σ :=
-    inf_chaselev_deque_lock γ_lock ∗
-    (inf_chaselev_deque_state₂₁ front back pub ∨ inf_chaselev_deque_state₂₂ front back pub).
-  #[local] Definition inf_chaselev_deque_state γ_lock front back pub : iProp Σ :=
-    inf_chaselev_deque_state₁ front back pub ∨
-    inf_chaselev_deque_state₂ γ_lock front back pub.
-
-  #[local] Definition inf_chaselev_deque_data_model data hist pub priv :=
-    array.(inf_array_model) data (
-      λ i,
-        let vs := hist ++ pub in
-        if decide (i < length vs) then vs !!! i else priv (i - length vs)
-    ).
-
-  #[local] Definition inf_chaselev_deque_inv_inner l γ_ctl γ_front γ_hist γ_pub γ_lock data : iProp Σ :=
-    ∃ front back hist pub priv,
-    (* physical fields *)
-    l.(front) ↦ #front ∗ l.(back) ↦ #back ∗
-    (* control token *)
-    inf_chaselev_deque_ctl₁ γ_ctl back priv ∗
-    (* front authority *)
-    inf_chaselev_deque_front_auth γ_front front ∗
-    (* data model *)
-    inf_chaselev_deque_data_model data hist pub priv ∗
-    (* history values *)
-    ⌜length hist = front⌝ ∗
-    inf_chaselev_deque_hist_auth γ_hist hist pub ∗
-    (* public values *)
-    inf_chaselev_deque_pub₁ γ_pub pub ∗
-    (* state *)
-    inf_chaselev_deque_state γ_lock front back pub.
-  Definition inf_chaselev_deque_inv t ι : iProp Σ :=
-    ∃ l γ_ctl γ_front γ_hist γ_pub γ_lock data,
-    ⌜t = #l⌝ ∗
-    (* metas *)
-    meta l inf_chaselev_deque_meta_ctl γ_ctl ∗
-    meta l inf_chaselev_deque_meta_front γ_front ∗
-    meta l inf_chaselev_deque_meta_hist γ_hist ∗
-    meta l inf_chaselev_deque_meta_pub γ_pub ∗
-    meta l inf_chaselev_deque_meta_lock γ_lock ∗
-    (* physical fields *)
-    l.(data) ↦□ data ∗
-    (* invariant *)
-    inv ι (inf_chaselev_deque_inv_inner l γ_ctl γ_front γ_hist γ_pub γ_lock data).
+  #[local] Definition inf_chaselev_deque_winner₁ γ_winner front Φ :=
+    auth_excl_frag (auth_excl_G := inf_chaselev_deque_G_winner_G) γ_winner (front, Next ∘ Φ).
+  #[local] Definition inf_chaselev_deque_winner₂ γ_winner front Φ :=
+    auth_excl_auth (auth_excl_G := inf_chaselev_deque_G_winner_G) γ_winner (DfracOwn 1) (front, Next ∘ Φ).
+  #[local] Definition inf_chaselev_deque_winner γ_winner : iProp Σ :=
+    ∃ front Φ1 Φ2,
+    inf_chaselev_deque_winner₁ γ_winner front Φ1 ∗
+    inf_chaselev_deque_winner₂ γ_winner front Φ2.
 
   Definition inf_chaselev_deque_model t pub : iProp Σ :=
     ∃ l γ_pub,
@@ -232,11 +240,118 @@ Section inf_chaselev_deque_G.
     (* lock *)
     inf_chaselev_deque_lock γ_lock.
 
-  #[global] Instance inf_chaselev_deque_inv_persistent t ι :
-    Persistent (inf_chaselev_deque_inv t ι).
-  Proof.
-    apply _.
-  Qed.
+  #[local] Definition inf_chaselev_deque_atomic_update γ_pub ι Φ : iProp Σ :=
+    AU << ∃∃ pub,
+      inf_chaselev_deque_pub₂ γ_pub pub
+    >>
+      @ ⊤ ∖ ↑ι, ∅
+    << ∀∀ v pub',
+      ⌜pub = v :: pub'⌝ ∗ inf_chaselev_deque_pub₂ γ_pub pub',
+      COMM Φ (SOMEV v)
+    >>.
+  #[local] Definition inf_chaselev_deque_state_inner₁ γ_winner :=
+    inf_chaselev_deque_winner γ_winner.
+  #[local] Definition inf_chaselev_deque_state₁ γ_hist γ_winner front back hist : iProp Σ :=
+    (* physical configuration *)
+    ⌜Z.of_nat front = back⌝ ∗
+    (* history values *)
+    inf_chaselev_deque_hist_auth γ_hist hist ∗
+    ⌜length hist = front⌝ ∗
+    (* inner state *)
+    inf_chaselev_deque_state_inner₁ γ_winner.
+  #[local] Definition inf_chaselev_deque_state_inner₂ γ_pub γ_winner ι front prophs : iProp Σ :=
+    match filter (λ '(_, _, front', _), front' = front) prophs with
+    | [] =>
+        inf_chaselev_deque_winner γ_winner
+    | (_, _, _, id) :: _ =>
+          inf_chaselev_deque_winner γ_winner
+        ∨ identifier_model id ∗
+          ∃ Φ,
+          inf_chaselev_deque_winner₁ γ_winner front Φ ∗
+          inf_chaselev_deque_atomic_update γ_pub ι Φ
+    end.
+  #[local] Definition inf_chaselev_deque_state₂ γ_hist γ_pub γ_winner ι front back hist pub prophs : iProp Σ :=
+    (* physical configuration *)
+    ⌜(front < back)%Z⌝ ∗
+    (* history values *)
+    inf_chaselev_deque_hist_auth γ_hist (hist ++ [pub !!! 0]) ∗
+    ⌜length hist = front⌝ ∗
+    (* inner state *)
+    inf_chaselev_deque_state_inner₂ γ_pub γ_winner ι front prophs.
+  #[local] Definition inf_chaselev_deque_state_inner₃₁ γ_winner front hist prophs : iProp Σ :=
+    match filter (λ '(_, _, front', _), front' = front) prophs with
+    | [] =>
+        inf_chaselev_deque_winner γ_winner
+    | (_, _, _, id) :: _ =>
+          inf_chaselev_deque_winner γ_winner
+        ∨ identifier_model id ∗
+          ∃ Φ,
+          inf_chaselev_deque_winner₁ γ_winner front Φ ∗
+          Φ (SOMEV (hist !!! front))
+    end.
+  #[local] Definition inf_chaselev_deque_state₃₁ γ_hist γ_winner front back hist prophs : iProp Σ :=
+    (* physical configuration *)
+    ⌜Z.of_nat front = back⌝ ∗
+    (* history values *)
+    inf_chaselev_deque_hist_auth γ_hist hist ∗
+    ⌜length hist = S front⌝ ∗
+    (* inner state *)
+    inf_chaselev_deque_state_inner₃₁ γ_winner front hist prophs.
+  #[local] Definition inf_chaselev_deque_state_inner₃₂ γ_winner :=
+    inf_chaselev_deque_winner γ_winner.
+  #[local] Definition inf_chaselev_deque_state₃₂ γ_hist γ_winner front back hist : iProp Σ :=
+    (* physical configuration *)
+    ⌜Z.of_nat front = (back + 1)%Z⌝ ∗
+    (* history values *)
+    inf_chaselev_deque_hist_auth γ_hist hist ∗
+    ⌜length hist = front⌝ ∗
+    (* inner state *)
+    inf_chaselev_deque_state_inner₃₂ γ_winner.
+  #[local] Definition inf_chaselev_deque_state₃ γ_hist γ_lock γ_winner front back hist pub prophs : iProp Σ :=
+    inf_chaselev_deque_lock γ_lock ∗
+    ( inf_chaselev_deque_state₃₁ γ_hist γ_winner front back hist prophs
+    ∨ inf_chaselev_deque_state₃₂ γ_hist γ_winner front back hist
+    ).
+  #[local] Definition inf_chaselev_deque_state γ_hist γ_pub γ_lock γ_winner ι front back hist pub prophs : iProp Σ :=
+      inf_chaselev_deque_state₁ γ_hist γ_winner front back hist
+    ∨ inf_chaselev_deque_state₂ γ_hist γ_pub γ_winner ι front back hist pub prophs
+    ∨ inf_chaselev_deque_state₃ γ_hist γ_lock γ_winner front back hist pub prophs.
+
+  #[local] Definition inf_chaselev_deque_inv_inner l γ_ctl γ_front γ_hist γ_pub γ_lock γ_prophet γ_winner ι data p : iProp Σ :=
+    ∃ front back hist pub priv past prophs,
+    (* mutable physical fields *)
+    l.(front) ↦ #front ∗ l.(back) ↦ #back ∗
+    (* control token *)
+    inf_chaselev_deque_ctl₁ γ_ctl back priv ∗
+    (* front authority *)
+    inf_chaselev_deque_front_auth γ_front front ∗
+    (* data model *)
+    array.(inf_array_model') data (hist ++ pub) priv ∗
+    (* public values *)
+    inf_chaselev_deque_pub₁ γ_pub pub ∗
+    ⌜length pub = Z.to_nat (back - front)⌝ ∗
+    (* prophet model *)
+    wise_prophet_model inf_chaselev_deque_prophet p γ_prophet past prophs ∗
+    ⌜Forall (λ '(_, _, front', _), front' < front) past⌝ ∗
+    (* state *)
+    inf_chaselev_deque_state γ_hist γ_pub γ_lock γ_winner ι front back hist pub prophs.
+  Definition inf_chaselev_deque_inv t ι : iProp Σ :=
+    ∃ l γ_ctl γ_front γ_hist γ_pub γ_lock γ_prophet γ_winner data p,
+    ⌜t = #l⌝ ∗
+    (* metas *)
+    meta l inf_chaselev_deque_meta_ctl γ_ctl ∗
+    meta l inf_chaselev_deque_meta_front γ_front ∗
+    meta l inf_chaselev_deque_meta_hist γ_hist ∗
+    meta l inf_chaselev_deque_meta_pub γ_pub ∗
+    meta l inf_chaselev_deque_meta_lock γ_lock ∗
+    meta l inf_chaselev_deque_meta_prophet γ_prophet ∗
+    meta l inf_chaselev_deque_meta_winner γ_winner ∗
+    (* immutable physical fields *)
+    l.(data) ↦□ data ∗
+    l.(prophecy) ↦□ #p ∗
+    (* main invariant *)
+    inv ι (inf_chaselev_deque_inv_inner l γ_ctl γ_front γ_hist γ_pub γ_lock γ_prophet γ_winner ι data p).
+
   #[global] Instance inf_chaselev_deque_model_timeless t pub :
     Timeless (inf_chaselev_deque_model t pub).
   Proof.
@@ -247,13 +362,18 @@ Section inf_chaselev_deque_G.
   Proof.
     apply _.
   Qed.
+  #[global] Instance inf_chaselev_deque_inv_persistent t ι :
+    Persistent (inf_chaselev_deque_inv t ι).
+  Proof.
+    apply _.
+  Qed.
 
   #[local] Lemma inf_chaselev_deque_ctl_alloc :
     ⊢ |==> ∃ γ_ctl,
       inf_chaselev_deque_ctl₁ γ_ctl 0 (λ _, #()) ∗
       inf_chaselev_deque_ctl₂ γ_ctl 0 (λ _, #()).
   Proof.
-    iMod (auth_excl_alloc' (auth_excl_G := inf_chaselev_deque_G_ctl_G) ((0%Z, λ _, #()) : prodO ZO (nat -d> valO))) as "(%γ_ctl & Hctl₁ & Hctl₂)".
+    iMod (auth_excl_alloc' (auth_excl_G := inf_chaselev_deque_G_ctl_G) (0%Z, λ _, #())) as "(%γ_ctl & Hctl₁ & Hctl₂)".
     iExists γ_ctl. iFrame. done.
   Qed.
   #[local] Lemma inf_chaselev_deque_ctl_agree γ_ctl back1 priv1 back2 priv2 :
@@ -304,13 +424,35 @@ Section inf_chaselev_deque_G.
     iApply auth_nat_max_frag_get.
   Qed.
 
-  (* TODO: hist lemmas *)
   #[local] Lemma inf_chaselev_deque_hist_alloc :
     ⊢ |==> ∃ γ_hist,
-      inf_chaselev_deque_hist_auth γ_hist [] [].
+      inf_chaselev_deque_hist_auth γ_hist [].
   Proof.
     iMod (mono_list_alloc []) as "(%γ_hist & Hhist_auth & _)".
     iExists γ_hist. done.
+  Qed.
+  #[local] Lemma inf_chaselev_deque_hist_frag_get {γ_hist hist} i v :
+    hist !! i = Some v →
+    inf_chaselev_deque_hist_auth γ_hist hist -∗
+    inf_chaselev_deque_hist_frag γ_hist i v.
+  Proof.
+    iIntros "% Hhist_auth".
+    iDestruct (mono_list_lb_get with "Hhist_auth") as "#Hhist_frag".
+    iApply (mono_list_mapsto_get with "Hhist_frag"). done.
+  Qed.
+  #[local] Lemma inf_chaselev_deque_hist_agree γ_hist hist i v :
+    inf_chaselev_deque_hist_auth γ_hist hist -∗
+    inf_chaselev_deque_hist_frag γ_hist i v -∗
+    ⌜hist !! i = Some v⌝.
+  Proof.
+    apply mono_list_auth_mapsto_lookup.
+  Qed.
+  #[local] Lemma inf_chaselev_deque_hist_update {γ_hist hist} v :
+    inf_chaselev_deque_hist_auth γ_hist hist ==∗
+    inf_chaselev_deque_hist_auth γ_hist (hist ++ [v]).
+  Proof.
+    iIntros "Hhist_auth".
+    iMod (mono_list_auth_update_app [v] with "Hhist_auth") as "($ & _)". done.
   Qed.
 
   #[local] Lemma inf_chaselev_deque_pub_alloc :
@@ -353,13 +495,82 @@ Section inf_chaselev_deque_G.
   Proof.
     apply excl_exclusive.
   Qed.
-  #[local] Lemma inf_chaselev_deque_lock_state γ_lock front back pub :
+  #[local] Lemma inf_chaselev_deque_lock_state γ_hist γ_pub γ_lock γ_winner ι front back hist pub prophs :
     inf_chaselev_deque_lock γ_lock -∗
-    inf_chaselev_deque_state γ_lock front back pub -∗
-    inf_chaselev_deque_state₁ front back pub.
+    inf_chaselev_deque_state γ_hist γ_pub γ_lock γ_winner ι front back hist pub prophs -∗
+      inf_chaselev_deque_lock γ_lock ∗
+      ( inf_chaselev_deque_state₁ γ_hist γ_winner front back hist
+      ∨ inf_chaselev_deque_state₂ γ_hist γ_pub γ_winner ι front back hist pub prophs
+      ).
   Proof.
-    iIntros "Hlock [Hstate | (Hlock' & Hstate)]"; first done.
+    iIntros "Hlock [Hstate | [Hstate | (Hlock' & Hstate)]]"; [iFrame.. |].
     iDestruct (inf_chaselev_deque_lock_exclusive with "Hlock Hlock'") as %[].
+  Qed.
+
+  #[local] Lemma inf_chaselev_deque_winner_alloc :
+    ⊢ |==> ∃ γ_winner,
+      inf_chaselev_deque_winner γ_winner.
+  Proof.
+  Admitted.
+  #[local] Lemma inf_chaselev_deque_winner₂_exclusive γ_winner front Φ :
+    inf_chaselev_deque_winner₂ γ_winner front Φ -∗
+    inf_chaselev_deque_winner γ_winner -∗
+    False.
+  Proof.
+  Admitted.
+  #[local] Lemma inf_chaselev_deque_winner_agree {γ_winner front1 Φ1 front2 Φ2} v :
+    inf_chaselev_deque_winner₁ γ_winner front1 Φ1 -∗
+    inf_chaselev_deque_winner₂ γ_winner front2 Φ2 -∗
+      ⌜front1 = front2⌝ ∗
+      ▷ (Φ1 v ≡ Φ2 v) ∗
+      inf_chaselev_deque_winner₁ γ_winner front1 Φ1 ∗
+      inf_chaselev_deque_winner₂ γ_winner front1 Φ2.
+  Proof.
+  Admitted.
+  #[local] Lemma inf_chaselev_deque_winner_update {γ_winner front1 Φ1 front2 Φ2} front Φ :
+    inf_chaselev_deque_winner₁ γ_winner front1 Φ1 -∗
+    inf_chaselev_deque_winner₂ γ_winner front2 Φ2 ==∗
+      inf_chaselev_deque_winner₁ γ_winner front Φ ∗
+      inf_chaselev_deque_winner₂ γ_winner front Φ.
+  Proof.
+  Admitted.
+  #[local] Lemma inf_chaselev_deque_winner₂_state_inner₂ {γ_winner γ_pub ι front1 front2 prophs Φ} v :
+    inf_chaselev_deque_winner₂ γ_winner front1 Φ -∗
+    inf_chaselev_deque_state_inner₂ γ_pub γ_winner ι front2 prophs -∗
+      ∃ id Φ',
+      ⌜front1 = front2⌝ ∗
+      ▷ (Φ' v ≡ Φ v) ∗
+      inf_chaselev_deque_winner₁ γ_winner front1 Φ' ∗
+      inf_chaselev_deque_winner₂ γ_winner front1 Φ ∗
+      identifier_model id ∗
+      inf_chaselev_deque_atomic_update γ_pub ι Φ'.
+  Proof.
+    iIntros "Hwinner₂ Hstate".
+    rewrite /inf_chaselev_deque_state_inner₂. destruct (filter _ _) as [| (((? & ?) & ?) & id) prophs'] eqn:?.
+    - iDestruct (inf_chaselev_deque_winner₂_exclusive with "Hwinner₂ Hstate") as %[].
+    - iDestruct "Hstate" as "[Hwinner | (Hid & %Φ' & Hwinner₁ & HΦ')]".
+      + iDestruct (inf_chaselev_deque_winner₂_exclusive with "Hwinner₂ Hwinner") as %[].
+      + iDestruct (inf_chaselev_deque_winner_agree v with "Hwinner₁ Hwinner₂") as "(-> & Heq & Hwinner₁ & Hwinner₂)".
+        iExists id, Φ'. iFrame. done.
+  Qed.
+  #[local] Lemma inf_chaselev_deque_winner₂_state_inner₃₁ {γ_winner front1 front2 hist prophs Φ} v :
+    inf_chaselev_deque_winner₂ γ_winner front1 Φ -∗
+    inf_chaselev_deque_state_inner₃₁ γ_winner front2 hist prophs -∗
+      ∃ id Φ',
+      ⌜front1 = front2⌝ ∗
+      ▷ (Φ' v ≡ Φ v) ∗
+      inf_chaselev_deque_winner₁ γ_winner front1 Φ' ∗
+      inf_chaselev_deque_winner₂ γ_winner front1 Φ ∗
+      identifier_model id ∗
+      Φ' (SOMEV (hist !!! front1)).
+  Proof.
+    iIntros "Hwinner₂ Hstate".
+    rewrite /inf_chaselev_deque_state_inner₃₁. destruct (filter _ _) as [| (((? & ?) & ?) & id) prophs'] eqn:?.
+    - iDestruct (inf_chaselev_deque_winner₂_exclusive with "Hwinner₂ Hstate") as %[].
+    - iDestruct "Hstate" as "[Hwinner | (Hid & %Φ' & Hwinner₁ & HΦ')]".
+      + iDestruct (inf_chaselev_deque_winner₂_exclusive with "Hwinner₂ Hwinner") as %[].
+      + iDestruct (inf_chaselev_deque_winner_agree v with "Hwinner₁ Hwinner₂") as "(-> & Heq & Hwinner₁ & Hwinner₂)".
+        iExists id, Φ'. iFrame. done.
   Qed.
 
   Lemma inf_chaselev_deque_owner_exclusive t :
@@ -367,8 +578,8 @@ Section inf_chaselev_deque_G.
     inf_chaselev_deque_owner t -∗
     False.
   Proof.
-    iIntros "(%l1 & %γ_ctl1 & %γ_lock1 & %back1 & %priv1 & %Heq1 & #Hmeta_ctl1 & #Hmeta_lock1 & Hctl₂1 & Hlock1) (%l2 & %γ_ctl2 & %γ_lock2 & %back2 & %priv2 & %Heq2 & #Hmeta_ctl2 & #Hmeta_lock2 & Hctl₂2 & Hlock2)". simplify.
-    iDestruct (meta_agree with "Hmeta_lock1 Hmeta_lock2") as %->.
+    iIntros "(%l & %γ_ctl & %γ_lock & %back & %priv & -> & #Hmeta_ctl & #Hmeta_lock & Hctl₂1 & Hlock1) (%_l & %_γ_ctl & %_γ_lock & %_back & %_priv & %Heq & #_Hmeta_ctl & #_Hmeta_lock & Hctl₂2 & Hlock2)". injection Heq as <-.
+    iDestruct (meta_agree with "Hmeta_lock _Hmeta_lock") as %->.
     iApply (inf_chaselev_deque_lock_exclusive with "Hlock1 Hlock2").
   Qed.
 
@@ -377,7 +588,9 @@ Section inf_chaselev_deque_G.
       inf_chaselev_deque_make #()
     {{{ t,
       RET t;
-      inf_chaselev_deque_inv t ι ∗ inf_chaselev_deque_model t [] ∗ inf_chaselev_deque_owner t
+      inf_chaselev_deque_inv t ι ∗
+      inf_chaselev_deque_model t [] ∗
+      inf_chaselev_deque_owner t
     }}}.
   Proof.
     iIntros "%Φ _ HΦ".
@@ -385,33 +598,45 @@ Section inf_chaselev_deque_G.
     wp_apply (wp_allocN with "[//]"); first done. iIntros "%l (Hl & (Hmeta & _))".
     iDestruct (array_cons with "Hl") as "(Hfront & Hl)".
     iDestruct (array_cons with "Hl") as "(Hback & Hl)".
-    iDestruct (array_cons with "Hl") as "(Hdata & _)".
-    rewrite loc_add_0 -{2}(loc_add_0 l) loc_add_assoc /=. assert (1 + 1 = 2)%Z as -> by lia.
+    iDestruct (array_cons with "Hl") as "(Hdata & Hl)".
+    iDestruct (array_cons with "Hl") as "(Hp & _)".
+    rewrite loc_add_0 -{2}(loc_add_0 l) !loc_add_assoc /=.
+    assert (1 + 1 = 2)%Z as -> by lia.
+    assert (2 + 1 = 3)%Z as -> by lia.
     wp_pures.
     wp_apply (inf_array_make_spec with "[//]"). iIntros "%data Hdata_model".
     wp_pures. wp_store.
+    wp_apply (wise_prophet_new_proph_spec with "[//]"). iIntros "%p %γ_prophet %prophs Hprophet_model".
+    wp_pures. wp_store.
     iMod (mapsto_persist with "Hdata") as "#Hdata".
+    iMod (mapsto_persist with "Hp") as "#Hp".
     iApply "HΦ".
     iMod inf_chaselev_deque_ctl_alloc as "(%γ_ctl & Hctl₁ & Hctl₂)".
     iMod inf_chaselev_deque_front_alloc as "(%γ_front & Hfront_auth)".
     iMod inf_chaselev_deque_hist_alloc as "(%γ_hist & Hhist_auth)".
     iMod inf_chaselev_deque_pub_alloc as "(%γ_pub & Hpub₁ & Hpub₂)".
     iMod inf_chaselev_deque_lock_alloc as "(%γ_lock & Hlock)".
+    iMod inf_chaselev_deque_winner_alloc as "(%γ_winner & Hwinner)".
     iDestruct (meta_token_difference _ (↑inf_chaselev_deque_meta_ctl) with "Hmeta") as "(Hmeta_ctl & Hmeta)"; first solve_ndisj.
     iDestruct (meta_token_difference _ (↑inf_chaselev_deque_meta_front) with "Hmeta") as "(Hmeta_front & Hmeta)"; first solve_ndisj.
     iDestruct (meta_token_difference _ (↑inf_chaselev_deque_meta_hist) with "Hmeta") as "(Hmeta_hist & Hmeta)"; first solve_ndisj.
     iDestruct (meta_token_difference _ (↑inf_chaselev_deque_meta_pub) with "Hmeta") as "(Hmeta_pub & Hmeta)"; first solve_ndisj.
     iDestruct (meta_token_difference _ (↑inf_chaselev_deque_meta_lock) with "Hmeta") as "(Hmeta_lock & Hmeta)"; first solve_ndisj.
+    iDestruct (meta_token_difference _ (↑inf_chaselev_deque_meta_prophet) with "Hmeta") as "(Hmeta_prophet & Hmeta)"; first solve_ndisj.
+    iDestruct (meta_token_difference _ (↑inf_chaselev_deque_meta_winner) with "Hmeta") as "(Hmeta_winner & _)"; first solve_ndisj.
     iMod (meta_set _ _ γ_ctl with "Hmeta_ctl") as "#Hmeta_ctl"; first done.
     iMod (meta_set _ _ γ_front with "Hmeta_front") as "#Hmeta_front"; first done.
     iMod (meta_set _ _ γ_hist with "Hmeta_hist") as "#Hmeta_hist"; first done.
     iMod (meta_set _ _ γ_pub with "Hmeta_pub") as "#Hmeta_pub"; first done.
     iMod (meta_set _ _ γ_lock with "Hmeta_lock") as "#Hmeta_lock"; first done.
+    iMod (meta_set _ _ γ_prophet with "Hmeta_prophet") as "#Hmeta_prophet"; first done.
+    iMod (meta_set _ _ γ_winner with "Hmeta_winner") as "#Hmeta_winner"; first done.
     iSplitR "Hctl₂ Hpub₂ Hlock".
-    { iExists l, γ_ctl, γ_front, γ_hist, γ_pub, γ_lock, data. iFrame "∗#". iSplitR; first done.
-      iApply inv_alloc. iNext. iExists 0, 0%Z, [], [], (λ _, #()). iFrame.
+    { repeat iExists _. iFrame "#∗". iSplitR; first done.
+      iApply inv_alloc. iExists 0, 0%Z, [], [], (λ _, #()), [], prophs. iFrame.
       iSplit; first done.
-      iLeft. naive_solver.
+      iSplit; first done.
+      iLeft. iFrame. done.
     }
     iSplitL "Hpub₂".
     { iExists l, γ_pub. naive_solver. }
@@ -420,7 +645,8 @@ Section inf_chaselev_deque_G.
 
   Lemma inf_chaselev_deque_push_spec t ι v :
     <<<
-      inf_chaselev_deque_inv t ι ∗ inf_chaselev_deque_owner t |
+      inf_chaselev_deque_inv t ι ∗
+      inf_chaselev_deque_owner t |
       ∀∀ pub, inf_chaselev_deque_model t pub
     >>>
       inf_chaselev_deque_push t v @ ↑ι
@@ -429,8 +655,7 @@ Section inf_chaselev_deque_G.
       RET #(); inf_chaselev_deque_owner t
     >>>.
   Proof.
-    iIntros "!> %Φ ((%l & %γ_ctl & %γ_front & %γ_hist & %γ_pub & %γ_lock & %data & -> & #Hmeta_ctl & #Hmeta_front & #Hmeta_hist & #Hmeta_pub & #Hmeta_lock & #Hdata & #Hinv) & (%l' & %_γ_ctl & %_γ_lock & %back & %priv & %Heq & #_Hmeta_ctl & #_Hmeta_lock & Hctl₂ & Hlock)) HΦ".
-    injection Heq as <-.
+    iIntros "!> %Φ ((%l & %γ_ctl & %γ_front & %γ_hist & %γ_pub & %γ_lock & %γ_prophet & %γ_winner & %data & %p & -> & #Hmeta_ctl & #Hmeta_front & #Hmeta_hist & #Hmeta_pub & #Hmeta_lock & #Hmeta_prophet & #Hmeta_winner & #Hdata & #Hp & #Hinv) & (%l' & %_γ_ctl & %_γ_lock & %back & %priv & %Heq & #_Hmeta_ctl & #_Hmeta_lock & Hctl₂ & Hlock)) HΦ". injection Heq as <-.
     iDestruct (meta_agree with "Hmeta_ctl _Hmeta_ctl") as %<-. iClear "_Hmeta_ctl".
     iDestruct (meta_agree with "Hmeta_lock _Hmeta_lock") as %<-. iClear "_Hmeta_lock".
 
@@ -439,16 +664,17 @@ Section inf_chaselev_deque_G.
     (* → [!#l.(back)] *)
     wp_bind (!#l.(back))%E.
     (* open invariant *)
-    iInv "Hinv" as "(%front & %_back & %hist & %pub & %_priv & Hfront & Hback & >Hctl₁ & Hfront_auth & Hdata_model & >%Hhist & Hhist_auth & Hpub₁ & Hstate)".
-    iDestruct (inf_chaselev_deque_ctl_agree with "Hctl₁ Hctl₂") as %?. simplify- front.
-    (* do load [back] *)
+    iInv "Hinv" as "(%front & %_back & %hist & %pub & %_priv & %past & %prophs & Hfront & Hback & >Hctl₁ & Hfront_auth & Hdata_model & Hpub₁ & >%Hpub & Hprophet_model & >%Hpast & Hstate)".
+    iDestruct (inf_chaselev_deque_ctl_agree with "Hctl₁ Hctl₂") as %(-> & ->).
+    (* do load back *)
     wp_load.
-    (* we have lock, hence we are in state 1 *)
-    iDestruct (inf_chaselev_deque_lock_state with "Hlock Hstate") as %Hstate.
-    (* hence, [0 ≤ back] *)
-    assert (0 ≤ back)%Z as Hback by lia.
+    (* we have lock, hence we are in state 1 or state 2, hence [0 ≤ back] *)
+    iAssert ⌜0 ≤ back⌝%I%Z as %Hback.
+    { iDestruct (inf_chaselev_deque_lock_state with "Hlock Hstate") as "(_ & [Hstate | Hstate])";
+        iDestruct "Hstate" as "(%Hstate & _)"; iPureIntro; lia.
+    }
     (* close invariant *)
-    iModIntro. iSplitL "Hfront Hback Hctl₁ Hfront_auth Hdata_model Hhist_auth Hpub₁ Hstate".
+    iModIntro. iSplitR "Hctl₂ Hlock HΦ".
     { repeat iExists _. iFrame. done. }
     clear- Hback.
 
@@ -457,96 +683,145 @@ Section inf_chaselev_deque_G.
     (* → [!#l.(data)] *)
     wp_load.
 
-    wp_pures.
-
     (* → [array.(inf_array_set) data #back v] *)
-    awp_apply (inf_array_set_spec with "[//]") without "HΦ"; first done.
+    awp_apply (inf_array_set_spec' with "[//]") without "HΦ"; first done.
     (* open invariant *)
-    iInv "Hinv" as "(%front & %_back & %hist & %pub & %_priv & Hfront & Hback & >Hctl₁ & Hfront_auth & >Hdata_model & >%Hhist & Hhist_auth & Hpub₁ & >Hstate)".
-    iDestruct (inf_chaselev_deque_ctl_agree with "Hctl₁ Hctl₂") as %?. simplify- front.
+    iInv "Hinv" as "(%front & %_back & %hist & %pub & %_priv & %past & %prophs & Hfront & Hback & >Hctl₁ & Hfront_auth & >Hdata_model & Hpub₁ & >%Hpub & Hprophet_model & >%Hpast & Hstate)".
+    iDestruct (inf_chaselev_deque_ctl_agree with "Hctl₁ Hctl₂") as %(-> & ->).
     iAaccIntro with "Hdata_model"; iIntros "Hdata_model".
-    { iModIntro. iFrame. repeat iExists _. iFrame. done. }
-    (* update [priv] in control tokens *)
+    { iFrame. repeat iExists _. iFrame. done. }
+    (* update private values in control tokens *)
     set (priv' := <[0 := v]> priv).
     iMod (inf_chaselev_deque_ctl_update back priv' with "Hctl₁ Hctl₂") as "(Hctl₁ & Hctl₂)".
-    (* we have lock, hence we are in state 1 *)
-    iDestruct (inf_chaselev_deque_lock_state with "Hlock Hstate") as %(Hstate & Hpub).
+    (* we have lock, hence we are in state 1 or state 2 *)
+    iDestruct (inf_chaselev_deque_lock_state with "Hlock Hstate") as "(Hlock & Hstate)".
+    (* hence [front ≤ back] and [length hist = front] *)
+    iAssert (◇ ⌜front ≤ back ∧ length hist = front⌝%Z)%I as "#>%".
+    { iDestruct "Hstate" as "[Hstate | Hstate]";
+        iDestruct "Hstate" as "(>%Hstate & _ & >%Hhist & _)";
+        iPureIntro; lia.
+    }
+    (* hence [back = length (hist ++ pub)] *)
+    assert (Z.to_nat back = length (hist ++ pub)) as Heq. { rewrite app_length. lia. }
+    rewrite Heq decide_False; last lia. rewrite Nat.sub_diag.
     (* close invariant *)
-    iModIntro. iSplitL "Hfront Hback Hctl₁ Hfront_auth Hdata_model Hhist_auth Hpub₁ Hstate".
-    { iNext. iExists front, back, hist, pub, priv'. iFrame. iSplit; last done.
-      (* update data *)
-      iApply (inf_array_model_proper with "Hdata_model").
-      intros i. rewrite app_length Hhist Hpub.
-      assert (front + Z.to_nat (back - front) = Z.to_nat back) as -> by lia.
-      destruct (Nat.lt_total i (Z.to_nat back)) as [| [-> |]].
-      - rewrite fn_lookup_insert_ne; last lia.
-        rewrite !decide_True //.
-      - rewrite fn_lookup_insert decide_False; last lia.
-        rewrite Nat.sub_diag //.
-      - rewrite fn_lookup_insert_ne; last lia.
-        rewrite !decide_False; [| lia..].
-        rewrite /priv' fn_lookup_insert_ne //. lia.
+    iModIntro. iSplitR "Hctl₂ Hlock".
+    { iExists front, back, hist, pub, priv', past, prophs. iFrame.
+      iSplit; first auto.
+      iSplit; first done.
+      iDestruct "Hstate" as "[Hstate | Hstate]"; [iLeft | iRight; iLeft]; done.
     }
     iIntros "_ HΦ".
-    clear- Hback.
+    clear.
 
     wp_pures.
 
     (* → [#l.(back) <- #(back + 1)] *)
     (* open invariant *)
-    iInv "Hinv" as "(%front & %_back & %hist & %pub & %_priv & Hfront & Hback & >Hctl₁ & Hfront_auth & Hdata_model & >%Hhist & Hhist_auth & Hpub₁ & Hstate)".
-    iDestruct (inf_chaselev_deque_ctl_agree with "Hctl₁ Hctl₂") as %?. simplify- front.
-    (* do increment [back] *)
+    iInv "Hinv" as "(%front & %_back & %hist & %pub & %_priv & %past & %prophs & Hfront & Hback & >Hctl₁ & Hfront_auth & Hdata_model & Hpub₁ & >%Hpub & Hprophet_model & >%Hpast & Hstate)".
+    iDestruct (inf_chaselev_deque_ctl_agree with "Hctl₁ Hctl₂") as %(-> & ->).
+    (* do increment back *)
     wp_store.
-    (* update [priv] in control tokens *)
-    set (priv'' := λ i, priv (S i)).
+    (* update private values in control tokens *)
+    set (priv'' i := priv (S i)).
     iMod (inf_chaselev_deque_ctl_update (back + 1) priv'' with "Hctl₁ Hctl₂") as "(Hctl₁ & Hctl₂)".
     (* begin transaction *)
-    iMod "HΦ" as "(%_pub & (%_l & %_γ_pub & %Heq & _Hmeta_pub & Hpub₂) & _ & HΦ)".
-    injection Heq as <-.
+    iMod "HΦ" as "(%_pub & (%_l & %_γ_pub & %Heq & _Hmeta_pub & Hpub₂) & _ & HΦ)". injection Heq as <-.
     iDestruct (meta_agree with "Hmeta_pub _Hmeta_pub") as %<-. iClear "_Hmeta_pub".
     iDestruct (inf_chaselev_deque_pub_agree with "Hpub₁ Hpub₂") as %<-.
-    (* update [pub] *)
+    (* update public values *)
     set (pub' := pub ++ [v]).
     iMod (inf_chaselev_deque_pub_update pub' with "Hpub₁ Hpub₂") as "(Hpub₁ & Hpub₂)".
     (* end transaction *)
     iMod ("HΦ" with "[Hpub₂]") as "HΦ".
-    { iExists l, γ_pub. iFrame "∗#". done. }
-    (* update [hist] *)
-    iAssert (inf_chaselev_deque_hist_auth γ_hist hist pub')%I with "[>Hhist_auth]" as "Hhist_auth".
-    { destruct pub; last done.
-      iMod (mono_list_auth_update_app [v] with "Hhist_auth") as "($ & _)". done.
-    }
-    (* we have lock, hence we are in state 1 *)
-    iDestruct (inf_chaselev_deque_lock_state with "Hlock Hstate") as %(Hstate & Hpub).
-    (* close invariant *)
-    iModIntro. iSplitL "Hfront Hback Hctl₁ Hfront_auth Hdata_model Hhist_auth Hpub₁ Hstate".
-    { iNext. iExists front, (back + 1)%Z, hist, pub', priv''. iFrame.
-      iSplitL "Hdata_model".
-      { (* update data *)
-        iApply (inf_array_model_proper with "Hdata_model").
-        intros i. rewrite /= !app_length /=.
-        destruct (Nat.lt_total i (length hist + length pub)) as [| [-> |]].
-        - rewrite !decide_True; [| lia..].
-          rewrite assoc lookup_total_app_l //. solve_length.
-        - rewrite decide_True; last lia.
-          rewrite decide_False; last lia.
-          rewrite Nat.sub_diag /priv' fn_lookup_insert.
-          rewrite assoc lookup_total_app_r; last solve_length.
-          rewrite app_length Nat.sub_diag //.
-        - rewrite !decide_False; [| lia..].
-          rewrite /priv' fn_lookup_insert_ne; last lia.
-          rewrite /priv''. f_equal. lia.
-      }
-      repeat iSplit; try done.
-      (* update state *)
-      iLeft. iPureIntro. split; [lia | rewrite app_length Hpub /=; lia].
-    }
-    clear.
+    { repeat iExists _. iFrame "#∗". done. }
+    (* update data model *)
+    iDestruct (inf_array_model'_shift_l with "Hdata_model") as "Hdata_model"; first by intros [].
+    rewrite -(assoc (++)) -/pub'.
+    (* we have lock, hence we are in state 1 or state 2 *)
+    iDestruct (inf_chaselev_deque_lock_state with "Hlock Hstate") as "(Hlock & [Hstate | Hstate])".
 
-    iApply "HΦ". repeat iExists _. iFrame "∗#". done.
+    - iDestruct "Hstate" as "(%Hstate & Hhist_auth & %Hhist & Hwinner)".
+      destruct (nil_or_length_pos pub) as [-> |]; last lia.
+      (* update history values *)
+      iMod (inf_chaselev_deque_hist_update v with "Hhist_auth") as "Hhist_auth".
+      (* close invariant *)
+      iModIntro. iSplitR "Hctl₂ Hlock HΦ".
+      { iExists front, (back + 1)%Z, hist, pub', priv'', past, prophs. iFrame.
+        iSplit. { iPureIntro. simpl. lia. }
+        iSplit; first done.
+        iRight. iLeft. iFrame. iSplit; first auto with lia.
+        rewrite /inf_chaselev_deque_state_inner₂. destruct (filter _ _) as [| (((_ & _) & _) & id) _]; auto.
+      }
+      clear.
+
+      iApply "HΦ". repeat iExists _. iFrame "#∗". done.
+
+    - iDestruct "Hstate" as "(%Hstate & Hhist_auth & %Hhist & Hwinner)".
+      destruct pub as [| w pub]; first naive_solver lia.
+      (* close invariant *)
+      iModIntro. iSplitR "Hctl₂ Hlock HΦ".
+      { iExists front, (back + 1)%Z, hist, pub', priv'', past, prophs. iFrame.
+        iSplit. { iPureIntro. rewrite app_length. simpl in *. lia. }
+        iSplit; first done.
+        iRight. iLeft. iFrame. iPureIntro. lia.
+      }
+      clear.
+
+      iApply "HΦ". repeat iExists _. iFrame "#∗". done.
   Qed.
 
+  #[local] Lemma inf_chaselev_deque_get_weak l γ_ctl γ_front γ_hist γ_pub γ_lock γ_prophet γ_winner ι data p (i : nat) :
+    {{{
+      inv ι (inf_chaselev_deque_inv_inner l γ_ctl γ_front γ_hist γ_pub γ_lock γ_prophet γ_winner ι data p) ∗
+      l.(data) ↦□ data
+    }}}
+      array.(inf_array_get) !#l.(data) #i
+    {{{ v, RET v; True }}}.
+  Proof.
+    iIntros "%Φ (#Hinv & #Hdata) HΦ".
+    wp_load.
+    awp_apply (inf_array_get_spec with "[//]") without "HΦ"; first lia.
+    iInv "Hinv" as "(%front & %back & %hist & %pub & %priv & %past & %prophs & Hfront & Hback & Hctl₁ & Hfront_auth & >Hdata_model & Hpub₁ & >%Hpub & Hprophet_model & >%Hpast & Hstate)".
+    iAaccIntro with "Hdata_model"; iIntros "Hdata_model".
+    { iModIntro. rewrite right_id. repeat iExists _. iFrame. done. }
+    iModIntro. iSplitL.
+    { repeat iExists _. iFrame. done. }
+    iIntros "_ HΦ". iApply ("HΦ" with "[//]").
+  Qed.
+  #[local] Lemma inf_chaselev_deque_get_strong l γ_ctl γ_front γ_hist γ_pub γ_lock γ_prophet γ_winner ι data p i v :
+    {{{
+      inv ι (inf_chaselev_deque_inv_inner l γ_ctl γ_front γ_hist γ_pub γ_lock γ_prophet γ_winner ι data p) ∗
+      l.(data) ↦□ data ∗
+      inf_chaselev_deque_hist_frag γ_hist i v
+    }}}
+      array.(inf_array_get) !#l.(data) #i
+    {{{ RET v; True }}}.
+  Proof.
+    iIntros "%Φ (#Hinv & #Hdata & #Hhist_frag) HΦ".
+    wp_load.
+    awp_apply (inf_array_get_spec with "[//]") without "HΦ"; first lia.
+    iInv "Hinv" as "(%front & %back & %hist & %pub & %priv & %past & %prophs & Hfront & Hback & Hctl₁ & Hfront_auth & >Hdata_model & Hpub₁ & >%Hpub & Hprophet_model & >%Hpast & Hstate)".
+    iAssert (◇ ⌜(hist ++ pub) !! i = Some v⌝)%I as "#>%Hlookup".
+    { iDestruct "Hstate" as "[(>%Hstate & >Hhist_auth & >%Hhist & _) | [(>%Hstate & >Hhist_auth & >%Hhist & _) | (_ & [(>%Hstate & >Hhist_auth & >%Hhist & _) | (>%Hstate & >Hhist_auth & >%Hhist & _)])]]";
+        iModIntro;
+        iDestruct (inf_chaselev_deque_hist_agree with "Hhist_auth Hhist_frag") as %?;
+        iPureIntro.
+      - erewrite lookup_app_l_Some; done.
+      - destruct pub as [| w pub]; simpl in *; first lia.
+        rewrite (assoc (++) hist [w]). erewrite lookup_app_l_Some; done.
+      - rewrite (nil_length_inv pub); last lia. list_simplifier. done.
+      - rewrite (nil_length_inv pub); last lia. erewrite lookup_app_l_Some; done.
+    }
+    iAaccIntro with "Hdata_model"; iIntros "Hdata_model".
+    { iModIntro. rewrite right_id. repeat iExists _. iFrame. done. }
+    iModIntro. iSplitL.
+    { repeat iExists _. iFrame. done. }
+    iIntros "_ HΦ".
+    rewrite Nat2Z.id decide_True; last eauto using lookup_lt_Some.
+    erewrite list_lookup_total_correct; last done.
+    iApply ("HΦ" with "[//]").
+  Qed.
   Lemma inf_chaselev_deque_steal_spec t ι :
     <<<
       inf_chaselev_deque_inv t ι |
@@ -555,25 +830,30 @@ Section inf_chaselev_deque_G.
       inf_chaselev_deque_steal t @ ↑ι
     <<<
       ∃∃ o,
-      (⌜length pub ≤ 1 ∧ o = NONEV⌝ ∗ inf_chaselev_deque_model t pub) ∨
-      (∃ pub' v, ⌜pub = v :: pub' ∧ o = SOMEV v⌝ ∗ inf_chaselev_deque_model t pub') |
+      (⌜pub = [] ∧ o = InjLV #()⌝ ∗ inf_chaselev_deque_model t []) ∨
+      (∃ v pub', ⌜pub = v :: pub' ∧ o = SOMEV v⌝ ∗ inf_chaselev_deque_model t pub') |
       RET o; True
     >>>.
   Proof.
-    iIntros "!> %Φ (%l & %γ_ctl & %γ_front & %γ_hist & %γ_pub & %γ_lock & %data & -> & #Hmeta_ctl & #Hmeta_front & #Hmeta_hist & #Hmeta_pub & #Hmeta_lock & #Hdata & #Hinv) HΦ".
-    iLöb as "HLöb".
+    iIntros "!> %Φ (%l & %γ_ctl & %γ_front & %γ_hist & %γ_pub & %γ_lock & %γ_prophet & %γ_winner & %data & %p & -> & #Hmeta_ctl & #Hmeta_front & #Hmeta_hist & #Hmeta_pub & #Hmeta_lock & #Hmeta_prophet & #Hmeta_winner & #Hdata & #Hp & #Hinv) HΦ".
+    iLöb as "IH".
 
     wp_rec. wp_pures.
+
+    (* → [NewId] *)
+    wp_apply (wp_new_id with "[//]"). iIntros "%id Hid".
+
+    wp_pures.
 
     (* → [!#l.(front)] *)
     wp_bind (!#l.(front))%E.
     (* open invariant *)
-    iInv "Hinv" as "(%front1 & %back1 & %hist & %pub & %priv & Hfront & Hback & Hctl₁ & Hfront_auth & Hdata_model & >%Hhist & Hhist_auth & Hpub₁ & Hstate)".
+    iInv "Hinv" as "(%front1 & %back1 & %hist & %pub & %priv & %past1 & %prophs1 & Hfront & Hback & Hctl₁ & Hfront_auth & Hdata_model & Hpub₁ & >%Hpub & Hprophet_model & >%Hpast & Hstate)".
     wp_load.
     (* emit front fragment at [front1] *)
     iDestruct (inf_chaselev_deque_front_frag_get with "Hfront_auth") as "#Hfront_frag".
     (* close invariant *)
-    iModIntro. iSplitL "Hfront Hback Hctl₁ Hfront_auth Hdata_model Hhist_auth Hpub₁ Hstate".
+    iModIntro. iSplitR "Hid HΦ".
     { repeat iExists _. iFrame. done. }
     clear.
 
@@ -582,19 +862,14 @@ Section inf_chaselev_deque_G.
     (* → [!#l.(back)] *)
     wp_bind (!#l.(back))%E.
     (* open invariant *)
-    iInv "Hinv" as "(%front2 & %back2 & %hist & %pub & %priv & Hfront & Hback & Hctl₁ & Hfront_auth & Hdata_model & >%Hhist & Hhist_auth & Hpub₁ & Hstate)".
+    iInv "Hinv" as "(%front2 & %back2 & %hist & %pub & %priv & %past2 & %prophs2 & Hfront & Hback & Hctl₁ & Hfront_auth & Hdata_model & Hpub₁ & >%Hpub & Hprophet_model & >%Hpast & Hstate)".
     wp_load.
+    (* we have [front1 ≤ front2] *)
+    iDestruct (inf_chaselev_deque_front_valid with "Hfront_auth Hfront_frag") as %Hfront2.
     (* enforce [front1 < back2] *)
-    destruct (decide (front1 < back2)%Z) as [Hbr1 | Hbr1]; last first.
-    { (* we have [1 ≤ length pub] *)
-      iAssert ⌜length pub ≤ 1⌝%I as %Hpub.
-      { iDestruct "Hstate" as "[%Hstate | (Hlock & [%Hstate | %Hstate])]".
-        - iDestruct (inf_chaselev_deque_front_valid with "Hfront_auth Hfront_frag") as %?.
-          destruct (decide (back2 = front1)) as [-> |]; last lia.
-          assert (front1 = front2) as <- by lia. iPureIntro. lia.
-        - iPureIntro. lia.
-        - simplify. auto.
-      }
+    destruct (decide (front1 < back2)%Z) as [Hbranch1 | Hbranch1]; last first.
+    { (* we have [pub = []] *)
+      assert (length pub = 0) as ->%nil_length_inv by lia.
       (* begin transaction *)
       iMod "HΦ" as "(%_pub & (%_l & %_γ_pub & %Heq & #_Hmeta_pub & Hpub₂) & _ & HΦ)". injection Heq as <-.
       iDestruct (meta_agree with "Hmeta_pub _Hmeta_pub") as %<-. iClear "_Hmeta_pub".
@@ -603,14 +878,9 @@ Section inf_chaselev_deque_G.
       iMod ("HΦ" with "[Hpub₂] [//]") as "HΦ".
       { iLeft. iSplit; first done. repeat iExists _. naive_solver. }
       (* close invariant *)
-      iModIntro. iSplitL "Hfront Hback Hctl₁ Hfront_auth Hdata_model Hhist_auth Hpub₁ Hstate".
+      iModIntro. iSplitR "Hid HΦ".
       { repeat iExists _. iFrame. done. }
-      clear- Hbr1.
-
-      wp_pures.
-
-      (* → [!#l.(data)] *)
-      wp_load.
+      clear- Hbranch1.
 
       wp_pures.
 
@@ -621,22 +891,14 @@ Section inf_chaselev_deque_G.
 
       iApply "HΦ".
     }
-    (* we have [front1 ≤ front2] *)
-    iDestruct (inf_chaselev_deque_front_valid with "Hfront_auth Hfront_frag") as %Hbr2.
     (* enforce [front2 = front1] *)
-    rewrite Nat.le_lteq in Hbr2. destruct Hbr2 as [Hbr2 | <-].
+    rewrite Nat.le_lteq in Hfront2. destruct Hfront2 as [Hbranch2 | <-].
     { (* emit front fragment at [front2] *)
-      iClear "Hfront_frag".
-      iDestruct (inf_chaselev_deque_front_frag_get with "Hfront_auth") as "#Hfront_frag".
+      iClear "Hfront_frag". iDestruct (inf_chaselev_deque_front_frag_get with "Hfront_auth") as "#Hfront_frag".
       (* close invariant *)
-      iModIntro. iSplitL "Hfront Hback Hctl₁ Hfront_auth Hdata_model Hhist_auth Hpub₁ Hstate".
+      iModIntro. iSplitR "Hid HΦ".
       { repeat iExists _. iFrame. done. }
-      clear- Hbr1 Hbr2.
-
-      wp_pures.
-
-      (* → [!#l.(data)] *)
-      wp_load.
+      clear- Hbranch1 Hbranch2.
 
       wp_pures.
 
@@ -645,61 +907,201 @@ Section inf_chaselev_deque_G.
 
       wp_pures.
 
-      (* → [array.(inf_array_get) data #front1] *)
-      awp_apply (inf_array_get_spec with "[//]")  without "HΦ"; first lia.
-      (* open invariant *)
-      iInv "Hinv" as "(%front3 & %back3 & %hist & %pub & %priv & Hfront & Hback & Hctl₁ & Hfront_auth & >Hdata_model & >%Hhist & Hhist_auth & Hpub₁ & Hstate)".
-      iAaccIntro with "Hdata_model"; iIntros "Hdata_model".
-      { iModIntro. rewrite right_id. repeat iExists _. iFrame. done. }
-      (* close invariant *)
-      iModIntro. iSplitL "Hfront Hback Hctl₁ Hfront_auth Hdata_model Hhist_auth Hpub₁ Hstate".
-      { repeat iExists _. iFrame. done. }
-      iIntros "_ HΦ".
-      remember (if decide _ then _ else _) as v.
-      clear- Hbr1 Hbr2.
+      (* → [array.(inf_array_get) !#l.(data) #front1] *)
+      wp_apply (inf_chaselev_deque_get_weak with "[$Hinv $Hdata]"). iIntros "%v _".
 
       wp_pures.
 
-      (* → [CmpXchg #l.(front) #front1 #(front1 + 1)] *)
-      wp_bind (CmpXchg #l.(front) #front1 #(front1 + 1)).
+      (* → [!#l.(prophecy)] *)
+      wp_load.
+
+      wp_pures.
+
+      (* → [Resolve (CmpXchg #l.(front) #front1 #(front1 + 1)) #p (#front1, #id)] *)
+      wp_bind (Resolve (CmpXchg #l.(front) #front1 #(front1 + 1)) #p (#front1, #id)%V).
       (* open invariant *)
-      iInv "Hinv" as "(%front4 & %back4 & %hist & %pub & %priv & Hfront & Hback & Hctl₁ & Hfront_auth & Hdata_model & >%Hhist & Hhist_auth & Hpub₁ & Hstate)".
-      (* CAS must fail as we have seen [front2] such that [front1 < front2] *)
-      wp_cmpxchg as ? | _.
-      { simplify- front1.
-        iDestruct (inf_chaselev_deque_front_valid with "Hfront_auth Hfront_frag") as %?.
+      iInv "Hinv" as "(%front3 & %back3 & %hist & %pub & %priv & %past3 & %prophs3 & Hfront & Hback & Hctl₁ & Hfront_auth & Hdata_model & Hpub₁ & >%Hpub & >Hprophet_model & >%Hpast & Hstate)".
+      (* do resolve *)
+      wp_apply (wise_prophet_resolve_spec with "Hprophet_model"); first done.
+      (* CmpXchg must fail as we have seen [front2] such that [front1 < front2] *)
+      wp_cmpxchg as [= ->%(inj _)] | _Hbranch3.
+      { iDestruct (inf_chaselev_deque_front_valid with "Hfront_auth Hfront_frag") as %?.
         lia.
       }
+      iAssert ⌜front1 < front3⌝%I as %Hbranch3; last clear _Hbranch3.
+      { iDestruct (inf_chaselev_deque_front_valid with "Hfront_auth Hfront_frag") as %?.
+        iPureIntro. lia.
+      }
+      iModIntro. iExists (front3, false, front1, id). iSplit; first done. iIntros "%prophs3' -> Hprophet_model".
       (* close invariant *)
-      iModIntro. iSplitL "Hfront Hback Hctl₁ Hfront_auth Hdata_model Hhist_auth Hpub₁ Hstate".
-      { repeat iExists _. iFrame. done. }
+      iModIntro. iSplitR "Hid HΦ".
+      { iExists front3, back3, hist, pub, priv, (past3 ++ [_]), prophs3'. iFrame.
+        iSplit; first done.
+        iSplit. { iPureIntro. decompose_Forall; done. }
+        iDestruct "Hstate" as "[Hstate | [(%Hstate & Hhist_auth & %Hhist & Hstate) | (Hlock & [(%Hstate & Hhist_auth & %Hhist & Hstate) | Hstate])]]".
+        - iLeft. done.
+        - iRight. iLeft. iFrame. iSplit; first done. iSplit; first done.
+          rewrite /inf_chaselev_deque_state_inner₂ filter_cons_False //. lia.
+        - do 2 iRight. iFrame. iLeft. iFrame. iSplit; first done. iSplit; first done.
+          rewrite /inf_chaselev_deque_state_inner₃₁ filter_cons_False //. lia.
+        - do 2 iRight. iFrame.
+      }
+      clear- Hbranch1 Hbranch2 Hbranch3.
 
       wp_pures.
 
       (* → [inf_chaselev_deque_steal #l] *)
-      wp_apply ("HLöb" with "HΦ").
+      wp_apply ("IH" with "HΦ").
     }
-    (* we are in state 1, hence [length pub = back2 - front1] *)
-    iAssert ⌜length pub = Z.to_nat (back2 - front1)⌝%I as %Hpub.
-    { iDestruct "Hstate" as "[% | (_ & [% | %])]"; [naive_solver | lia..]. }
-    (* hence, [pub] contains at least one value *)
+    (* we are in state 2 *)
+    iDestruct "Hstate" as "[(%Hstate & _) | [(_ & Hhist_auth & %Hhist & Hstate) | (_ & [(%Hstate & _) | (%Hstate & _)])]]"; try lia.
+    (* hence there is at least one public value *)
     destruct pub as [| v pub]; first naive_solver lia.
     (* emit history fragment at [front1] *)
-    iAssert (inf_chaselev_deque_hist_frag γ_hist front1 v) as "#Hhist_frag".
-    { iDestruct (mono_list_lb_get with "Hhist_auth") as "#Hhist_frag".
-      iApply (mono_list_mapsto_get with "Hhist_frag").
-      rewrite lookup_app_r; last lia.
-      rewrite Hhist Nat.sub_diag //.
+    iDestruct (inf_chaselev_deque_hist_frag_get front1 v with "Hhist_auth") as "#Hhist_frag".
+    { rewrite lookup_app_r; last lia. rewrite Hhist Nat.sub_diag //. }
+    (* emit prophet lower bound *)
+    iDestruct (wise_prophet_lb_get with "Hprophet_model") as "#Hprophet_lb".
+    (* enforce [filter (λ '(_, _, front', _), front' = front1) prophs2 ≠ []] *)
+    rewrite /inf_chaselev_deque_state_inner₂. destruct (filter _ prophs2) as [| (((front1' & b) & front1'') & id') prophs2'] eqn:Hbranch2.
+    { (* close invariant *)
+      iModIntro. iSplitR "Hid HΦ".
+      { iExists front1, back2, hist, (v :: pub), priv, past2, prophs2. iFrame.
+        iSplit; first done.
+        iSplit; first done.
+        iRight. iLeft. iFrame. iSplit; first done. iSplit; first done.
+        rewrite /inf_chaselev_deque_state_inner₂ Hbranch2 //.
+      }
+      clear- Hbranch1 Hbranch2.
+
+      wp_pures.
+
+      (* → [if: #(bool_decide (front1 < back2))] *)
+      rewrite bool_decide_eq_true_2; last done.
+
+      wp_pures.
+
+      (* → [array.(inf_array_get) !#l.(data) #front1] *)
+      wp_apply (inf_chaselev_deque_get_strong with "[$Hinv $Hdata $Hhist_frag]"). iIntros "_".
+
+      wp_pures.
+
+      (* → [!#l.(prophecy)] *)
+      wp_load.
+
+      wp_pures.
+
+      (* → [Resolve (CmpXchg #l.(front) #front1 #(front1 + 1)) #p (#front1, #id)] *)
+      wp_bind (Resolve (CmpXchg #l.(front) #front1 #(front1 + 1)) #p (#front1, #id)%V).
+      (* open invariant *)
+      iInv "Hinv" as "(%front3 & %back3 & %hist & %pub & %priv & %past3 & %prophs3 & Hfront & Hback & Hctl₁ & Hfront_auth & Hdata_model & Hpub₁ & >%Hpub & >Hprophet_model & >%Hpast & Hstate)".
+      (* current prophecies are a suffix of prophet lower bound *)
+      iDestruct (wise_prophet_model_lb_valid with "Hprophet_model Hprophet_lb") as %(past3_1 & past3_2 & -> & ->).
+      (* do resolve *)
+      wp_apply (wise_prophet_resolve_spec with "Hprophet_model"); first done.
+      (* whether CmpXchg succeed or not, we reach a contradiction *)
+      wp_cmpxchg as _ | _.
+      all: iModIntro; iExists (front3, _, front1, id); iSplit; first done; iIntros "%prophs3' ->".
+      all: eelim (filter_nil_not_elem_of _ _ (front3, _, front1, id)); [naive_solver.. |].
+      all: apply elem_of_app; right; apply elem_of_cons; left; naive_solver.
     }
+    (* enforce [id' = id] *)
+    destruct (decide (id' = id)) as [-> | Hbranch3]; first last.
+    { (* close invariant *)
+      iModIntro. iSplitR "Hid HΦ".
+      { iExists front1, back2, hist, (v :: pub), priv, past2, prophs2. iFrame.
+        iSplit; first done.
+        iSplit; first done.
+        iRight. iLeft. iFrame. iSplit; first done. iSplit; first done.
+        rewrite /inf_chaselev_deque_state_inner₂ Hbranch2 //.
+      }
+      clear- Hbranch1 Hbranch2 Hbranch3.
+
+      wp_pures.
+
+      (* → [if: #(bool_decide (front1 < back2))] *)
+      rewrite bool_decide_eq_true_2; last done.
+
+      wp_pures.
+
+      (* → [array.(inf_array_get) !#l.(data) #front1] *)
+      wp_apply (inf_chaselev_deque_get_strong with "[$Hinv $Hdata $Hhist_frag]"). iIntros "_".
+
+      wp_pures.
+
+      (* → [!#l.(prophecy)] *)
+      wp_load.
+
+      wp_pures.
+
+      (* → [Resolve (CmpXchg #l.(front) #front1 #(front1 + 1)) #p (#front1, #id)] *)
+      wp_bind (Resolve (CmpXchg #l.(front) #front1 #(front1 + 1)) #p (#front1, #id)%V).
+      (* open invariant *)
+      iInv "Hinv" as "(%front3 & %back3 & %hist & %pub & %priv & %past3 & %prophs3 & Hfront & Hback & Hctl₁ & Hfront_auth & Hdata_model & Hpub₁ & >%Hpub & >Hprophet_model & >%Hpast & Hstate)".
+      (* current prophecies are a suffix of prophet lower bound *)
+      iDestruct (wise_prophet_model_lb_valid with "Hprophet_model Hprophet_lb") as %(past3_1 & past3_2 & -> & ->).
+      (* do resolve *)
+      wp_apply (wise_prophet_resolve_spec with "Hprophet_model"); first done.
+      (* CmpXchg must fail as we are not the winner *)
+      wp_cmpxchg as [= ->%(inj _)] | _Hbranch4.
+      { iModIntro. iExists (front1, true, front1, id). iSplit; first done. iIntros "%prophs3' -> Hprophet_model".
+        exfalso. simpl in *.
+        rewrite filter_app filter_cons_True // in Hbranch2.
+        destruct (filter _ past3_2) as [| ? past3_2'] eqn:Heq; invert Hbranch2.
+        eassert ((front1', b, front1'', id') ∈ filter _ past3_2) as Helem.
+        { erewrite Heq. constructor. }
+        apply elem_of_list_filter in Helem as (-> & Helem).
+        rewrite Forall_app !Forall_forall in Hpast. destruct Hpast as (_ & Hpast).
+        specialize (Hpast (front1', b, front1, id') Helem). simpl in Hpast. lia.
+      }
+      iAssert ⌜front1 < front3⌝%I as %Hbranch4; last clear _Hbranch4.
+      { iDestruct (inf_chaselev_deque_front_valid with "Hfront_auth Hfront_frag") as %?.
+        iPureIntro. assert (front1 ≠ front3) by naive_solver. lia.
+      }
+      iModIntro. iExists (front3, false, front1, id). iSplit; first done. iIntros "%prophs3' -> Hprophet_model".
+      (* close invariant *)
+      iModIntro. iSplitR "Hid HΦ".
+      { iExists front3, back3, hist, pub, priv, _, prophs3'. iFrame.
+        iSplit; first done.
+        iSplit. { iPureIntro. decompose_Forall; done. }
+        iDestruct "Hstate" as "[Hstate | [(%Hstate & Hstate) | (Hlock & [(%Hstate & Hstate) | Hstate])]]".
+        - iLeft. done.
+        - iRight. iLeft. iFrame. iSplit; first done.
+          rewrite /inf_chaselev_deque_state_inner₂ filter_cons_False //. lia.
+        - do 2 iRight. iFrame. iLeft. iFrame. iSplit; first done.
+          rewrite /inf_chaselev_deque_state_inner₃₁ filter_cons_False //. lia.
+        - do 2 iRight. iFrame.
+      }
+      clear- Hbranch1 Hbranch2 Hbranch3 Hbranch4.
+
+      wp_pures.
+
+      (* → [inf_chaselev_deque_steal #l] *)
+      wp_apply ("IH" with "HΦ").
+    }
+    (* we now know we are the next winner *)
+    iDestruct "Hstate" as "[(% & % & % & Hwinner₁ & Hwinner₂) | (Hid' & _)]"; last first.
+    { iDestruct (identifier_model_exclusive with "Hid Hid'") as %[]. }
+    iMod (inf_chaselev_deque_winner_update front1 Φ with "Hwinner₁ Hwinner₂") as "(Hwinner₁ & Hwinner₂)".
     (* close invariant *)
-    iModIntro. iSplitL "Hfront Hback Hctl₁ Hfront_auth Hdata_model Hhist_auth Hpub₁ Hstate".
-    { repeat iExists _. iFrame. done. }
-    clear- Hbr1.
-
-    wp_pures.
-
-    (* → [!#l.(data)] *)
-    wp_load.
+    iModIntro. iSplitR "Hwinner₂".
+    { iExists front1, back2, hist, (v :: pub), priv, past2, prophs2. iFrame.
+      iSplit; first done.
+      iSplit; first done.
+      iRight. iLeft. iFrame. iSplit; first done. iSplit; first done.
+      rewrite /inf_chaselev_deque_state_inner₂ Hbranch2. iRight. iFrame. iExists Φ. iFrame.
+      iNext. rewrite /inf_chaselev_deque_atomic_update. iAuIntro.
+      iApply (aacc_aupd_commit with "HΦ"); first done. iIntros "%_pub (%_l & %_γ_pub & %Heq & #_Hmeta_pub & Hpub₂)". injection Heq as <-.
+      iDestruct (meta_agree with "Hmeta_pub _Hmeta_pub") as %<-.
+      iAaccIntro with "Hpub₂".
+      { iIntros "Hpub₂ !>". iSplitL "Hpub₂"; last auto.
+        repeat iExists _. iFrame "#∗". done.
+      }
+      iIntros "%w %pub' (-> & Hpub₂) !>". iExists (SOMEV w). iSplitL.
+      - iRight. repeat iExists _. iSplit; first done. repeat iExists _. iFrame "#∗". done.
+      - iIntros "HΦ". iApply ("HΦ" with "[//]").
+    }
+    clear- Hbranch1 Hbranch2.
 
     wp_pures.
 
@@ -708,139 +1110,115 @@ Section inf_chaselev_deque_G.
 
     wp_pures.
 
-    (* → [array.(inf_array_get) data #front1] *)
-    awp_apply (inf_array_get_spec with "[//]") without "HΦ"; first lia.
-    (* open invariant *)
-    iInv "Hinv" as "(%front3 & %back3 & %hist & %pub & %priv & Hfront & Hback & Hctl₁ & >Hfront_auth & >Hdata_model & >%Hhist & >Hhist_auth & Hpub₁ & Hstate)".
-    iAaccIntro with "Hdata_model"; iIntros "Hdata_model".
-    { iModIntro. rewrite right_id. repeat iExists _. iFrame. done. }
-    (* we have [front1 < front3] *)
-    iDestruct (inf_chaselev_deque_front_valid with "Hfront_auth Hfront_frag") as %Hbr3.
-    (* enforce [front3 = front1] *)
-    rewrite Nat.le_lteq in Hbr3. destruct Hbr3 as [Hbr3 | <-].
-    { (* emit front fragment at [front3] *)
-      iClear "Hfront_frag".
-      iDestruct (inf_chaselev_deque_front_frag_get with "Hfront_auth") as "#Hfront_frag".
-      (* close invariant *)
-      iModIntro. iSplitL "Hfront Hback Hctl₁ Hfront_auth Hdata_model Hhist_auth Hpub₁ Hstate".
-      { repeat iExists _. iFrame. done. }
-      iIntros "_ HΦ".
-      remember (if decide _ then _ else _) as w.
-      clear- Hbr1 Hbr3.
-
-      wp_pures.
-
-      (* → [CmpXchg #l.(front) #front1 #(front1 + 1)] *)
-      wp_bind (CmpXchg #l.(front) #front1 #(front1 + 1)).
-      (* open invariant *)
-      iInv "Hinv" as "(%front4 & %back4 & %hist & %pub & %priv & Hfront & Hback & Hctl₁ & Hfront_auth & Hdata_model & >%Hhist & Hhist_auth & Hpub₁ & Hstate)".
-      (* CAS must fail as we have seen [front3] such that [front1 < front3] *)
-      wp_cmpxchg as ? | _.
-      { simplify- front1.
-        iDestruct (inf_chaselev_deque_front_valid with "Hfront_auth Hfront_frag") as %?.
-        lia.
-      }
-      (* close invariant *)
-      iModIntro. iSplitL "Hfront Hback Hctl₁ Hfront_auth Hdata_model Hhist_auth Hpub₁ Hstate".
-      { repeat iExists _. iFrame. done. }
-
-      wp_pures.
-
-      (* → [inf_chaselev_deque_steal #l] *)
-      wp_apply ("HLöb" with "HΦ").
-    }
-    (* from history fragment at [front1], we know the loaded value is [v] *)
-    iDestruct (mono_list_auth_mapsto_lookup with "Hhist_auth Hhist_frag") as %Hhist_lookup.
-    replace (if decide _ then _ else _) with v; last first.
-    { destruct pub as [| w pub].
-      { rewrite list_lookup_alt in Hhist_lookup. lia. }
-      rewrite lookup_app_r in Hhist_lookup; last lia.
-      apply list_lookup_singleton_Some in Hhist_lookup as (_ & ->).
-      rewrite decide_True; last first.
-      { rewrite app_length /=. lia. }
-      rewrite lookup_total_app_r; last lia.
-      rewrite Nat2Z.id Hhist Nat.sub_diag //.
-    }
-    (* close invariant *)
-    iModIntro. iSplitL "Hfront Hback Hctl₁ Hfront_auth Hdata_model Hhist_auth Hpub₁ Hstate".
-    { repeat iExists _. iFrame. done. }
-    iIntros "_ HΦ".
-    clear- Hbr1.
+    (* → [array.(inf_array_get) !#l.(data) #front1] *)
+    wp_apply (inf_chaselev_deque_get_strong with "[$Hinv $Hdata $Hhist_frag]"). iIntros "_".
 
     wp_pures.
 
-    (* → [CmpXchg #l.(front) #front1 #(front1 + 1)] *)
-    wp_bind (CmpXchg #l.(front) #front1 #(front1 + 1)).
-    (* open invariant *)
-    iInv "Hinv" as "(%front4 & %back4 & %hist & %pub & %priv & Hfront & Hback & Hctl₁ & Hfront_auth & Hdata_model & >%Hhist & Hhist_auth & Hpub₁ & Hstate)".
-    (* begin transaction *)
-    iMod "HΦ" as "(%_pub & Hmodel & HΦ)".
-    wp_cmpxchg as ? | _; first last.
-    { (* abort transation *)
-      iMod ("HΦ" with "Hmodel") as "HΦ". iModIntro.
-      (* close invariant *)
-      iModIntro. iSplitL "Hfront Hback Hctl₁ Hfront_auth Hdata_model Hhist_auth Hpub₁ Hstate".
-      { repeat iExists _. iFrame. done. }
-
-      wp_pures.
-
-      (* → [inf_chaselev_deque_steal #l] *)
-      wp_apply ("HLöb" with "HΦ").
-    }
-    simplify- front1.
-    iDestruct "Hmodel" as "(%_l & %_γ_pub & %Heq & #_Hmeta_pub & Hpub₂)".
-    injection Heq as <-.
-    iDestruct (meta_agree with "Hmeta_pub _Hmeta_pub") as %<-. iClear "_Hmeta_pub".
-    iDestruct (inf_chaselev_deque_pub_agree with "Hpub₁ Hpub₂") as %<-.
-    (* [front] has not changed, hence [v] is still the front public value *)
-    iDestruct (mono_list_auth_mapsto_lookup with "Hhist_auth Hhist_frag") as %Hhist_lookup.
-    destruct pub as [| w pub].
-    { rewrite list_lookup_alt in Hhist_lookup. lia. }
-    rewrite lookup_app_r in Hhist_lookup; last lia.
-    apply list_lookup_singleton_Some in Hhist_lookup as (_ & ->).
-    (* end transation *)
-    iMod (inf_chaselev_deque_pub_update pub with "Hpub₁ Hpub₂") as "(Hpub₁ & Hpub₂)".
-    iAssert (inf_chaselev_deque_model #l pub) with "[Hpub₂]" as "Hmodel".
-    { iExists l, γ_pub. naive_solver. }
-    iMod ("HΦ" with "[Hmodel] [//]") as "HΦ"; first eauto. iModIntro.
-    (* update front authority *)
-    iMod (inf_chaselev_deque_front_auth_update (S front1) with "Hfront_auth") as "Hfront_auth"; first lia.
-    (* update [hist] *)
-    iAssert (inf_chaselev_deque_hist_auth γ_hist (hist ++ [v]) pub) with "[> Hhist_auth]" as "Hhist_auth".
-    { destruct pub as [| w pub]; first done.
-      iMod (mono_list_auth_update_app with "Hhist_auth") as "($ & _)". done.
-    }
-    (* update state *)
-    iAssert (inf_chaselev_deque_state γ_lock (S front1) back4 pub) with "[Hstate]" as "Hstate".
-    { iDestruct "Hstate" as "[%Hstate | (Hlock & [%Hstate | %Hstate])]".
-      - iLeft. naive_solver auto with lia.
-      - iRight. iFrame. iRight. iPureIntro.
-        split; first lia. rewrite -length_zero_iff_nil. list_simplifier. lia.
-      - naive_solver.
-    }
-    (* close invariant *)
-    iModIntro. iSplitL "Hfront Hback Hctl₁ Hfront_auth Hdata_model Hhist_auth Hpub₁ Hstate".
-    { iNext. iExists (S front1), back4, (hist ++ [v]), pub, priv. iFrame.
-      iSplitL "Hfront".
-      { replace (front1 + 1)%Z with (Z.of_nat (S front1)) by lia. done. }
-      iSplitL "Hdata_model".
-      { iApply (inf_array_model_proper with "Hdata_model").
-        intros i. rewrite /= !app_length /=. destruct (decide _).
-        - rewrite !decide_True; last lia. list_simplifier. done.
-        - rewrite !decide_False; last lia. rewrite -assoc //.
-      }
-      iPureIntro. rewrite app_length /= //. lia.
-    }
-    clear- Hbr1.
+    (* → [!#l.(prophecy)] *)
+    wp_load.
 
     wp_pures.
 
-    iApply "HΦ".
+    (* → [Resolve (CmpXchg #l.(front) #front1 #(front1 + 1)) #p (#front1, #id)] *)
+    wp_bind (Resolve (CmpXchg #l.(front) #front1 #(front1 + 1)) #p (#front1, #id)%V).
+    (* open invariant *)
+    iInv "Hinv" as "(%front3 & %back3 & %hist & %pub & %priv & %past3 & %prophs3 & Hfront & Hback & Hctl₁ & Hfront_auth & Hdata_model & Hpub₁ & >%Hpub & >Hprophet_model & >%Hpast & Hstate)".
+    (* we are in state 2 or state 3.1 *)
+    iDestruct "Hstate" as "[(_ & _ & _ & Hwinner) | [(>%Hbranch3 & Hhist_auth & >%Hhist & Hstate) | (Hlock & [(><- & Hhist_auth & >%Hhist & Hstate) | (_ & _ & _ & Hwinner)])]]";
+      (* do resolve *)
+      (wp_apply (wise_prophet_resolve_spec with "Hprophet_model"); first done).
+
+    1,4:
+      wp_cmpxchg as _ | _;
+      iDestruct (inf_chaselev_deque_winner₂_exclusive with "Hwinner₂ Hwinner") as %[].
+
+    - (* CmpXchg must succeed as we are the next winner *)
+      wp_cmpxchg as [= ->%(inj _)] | Hbranch4;
+        iDestruct (inf_chaselev_deque_winner₂_state_inner₂ (SOMEV v) with "Hwinner₂ Hstate") as "(%id' & %Φ' & %Heq & HΦ & Hwinner₁ & Hwinner₂ & _ & HΦ')";
+        [clear Heq | naive_solver].
+      iModIntro. iExists (front1, true, front1, id). iSplit; first done. iIntros "%prophs3' -> Hprophet_model".
+      (* update front *)
+      iMod (inf_chaselev_deque_front_auth_update (S front1) with "Hfront_auth") as "Hfront_auth"; first lia.
+      (* begin transaction *)
+      iMod "HΦ'" as "(%_pub & Hpub₂ & _ & HΦ')".
+      iDestruct (inf_chaselev_deque_pub_agree with "Hpub₁ Hpub₂") as %<-.
+      (* update public values *)
+      destruct pub as [| _v pub]; first naive_solver lia.
+      iAssert ⌜_v = v⌝%I as %->.
+      { iDestruct (inf_chaselev_deque_hist_agree with "Hhist_auth Hhist_frag") as %Hlookup.
+        iPureIntro.
+        rewrite lookup_app_r in Hlookup; last lia.
+        rewrite list_lookup_singleton_Some in Hlookup. naive_solver.
+      }
+      iMod (inf_chaselev_deque_pub_update pub with "Hpub₁ Hpub₂") as "(Hpub₁ & Hpub₂)".
+      (* end transaction *)
+      iMod ("HΦ'" with "[$Hpub₂ //]") as "HΦ'".
+      (* close invariant *)
+      iSplitR "HΦ HΦ'".
+      { simpl in Hpub.
+        iExists (S front1), back3, (hist ++ [v]), pub, priv, (past3 ++ [_]), prophs3'. iFrame.
+        iSplitL "Hfront". { assert (front1 + 1 = S front1)%Z as -> by lia. done. }
+        iSplitL "Hdata_model". { rewrite -(assoc (++)) //. }
+        iSplitR; first auto with lia.
+        iSplitR.
+        { iPureIntro. rewrite Forall_app Forall_singleton. split; last lia.
+          eapply Forall_impl; first done. intros (((? & ?) & ?) & ?) ?. lia.
+        }
+        destruct pub as [| w pub]; simpl in Hpub.
+        - iModIntro. iLeft. iFrame. iSplit; first auto with lia.
+          iSplit. { rewrite app_length /=. auto with lia. }
+          repeat iExists _. iFrame.
+        - iMod (inf_chaselev_deque_hist_update w with "Hhist_auth") as "Hhist_auth".
+          iModIntro. iRight. iLeft. iFrame. iSplit; first auto with lia.
+          iSplit. { rewrite app_length /=. auto with lia. }
+          rewrite /inf_chaselev_deque_state_inner₂. destruct (filter _ prophs3') as [| (((? & ?) & ?) & ?) ?].
+          + repeat iExists _. iFrame.
+          + iLeft. repeat iExists _. iFrame.
+      }
+      iModIntro.
+      clear- Hbranch1 Hbranch2 Hbranch3.
+
+      wp_pures.
+
+      iRewrite- "HΦ". done.
+
+    - (* CmpXchg must succeed as we are the next winner *)
+      wp_cmpxchg as [= ->%(inj _)] | Hbranch4;
+          iDestruct (inf_chaselev_deque_winner₂_state_inner₃₁ (SOMEV v) with "Hwinner₂ Hstate") as "(%id' & %Φ' & %Heq & HΦ & Hwinner₁ & Hwinner₂ & _ & HΦ')";
+        [clear Heq | naive_solver].
+      iModIntro. iExists (front1, true, front1, id). iSplit; first done. iIntros "%prophs3' -> Hprophet_model".
+      (* we know there is no public values and [hist !!! front1 = v] *)
+      destruct (nil_or_length_pos pub) as [-> |]; last lia.
+      iAssert ⌜hist !!! front1 = v⌝%I as %->.
+      { iDestruct (inf_chaselev_deque_hist_agree with "Hhist_auth Hhist_frag") as %Hlookup.
+        iPureIntro. apply list_lookup_total_correct. done.
+      }
+      (* update front *)
+      iMod (inf_chaselev_deque_front_auth_update (S front1) with "Hfront_auth") as "Hfront_auth"; first lia.
+      (* close invariant *)
+      iModIntro. iSplitR "HΦ HΦ'".
+      { iExists (S front1), front1, hist, [], priv, (past3 ++ [_]), prophs3'. iFrame.
+        iSplitL "Hfront". { assert (front1 + 1 = S front1)%Z as -> by lia. done. }
+        iSplit; first auto with lia.
+        iSplitR.
+        { iPureIntro. rewrite Forall_app Forall_singleton. split; last lia.
+          eapply Forall_impl; first done. intros (((? & ?) & ?) & ?) ?. lia.
+        }
+        do 2 iRight. iFrame. iRight. iSplit; first auto with lia. iSplit; first done.
+        repeat iExists _. iFrame.
+      }
+      clear- Hbranch1 Hbranch2.
+
+      wp_pures.
+
+      iRewrite- "HΦ". done.
   Qed.
 
   Lemma inf_chaselev_deque_pop_spec t ι :
     <<<
-      inf_chaselev_deque_inv t ι ∗ inf_chaselev_deque_owner t |
+      inf_chaselev_deque_inv t ι ∗
+      inf_chaselev_deque_owner t |
       ∀∀ pub, inf_chaselev_deque_model t pub
     >>>
       inf_chaselev_deque_pop t @ ↑ι
@@ -851,620 +1229,53 @@ Section inf_chaselev_deque_G.
       RET o; inf_chaselev_deque_owner t
     >>>.
   Proof.
-    iIntros "!> %Φ ((%l & %γ_ctl & %γ_front & %γ_hist & %γ_pub & %γ_lock & %data & -> & #Hmeta_ctl & #Hmeta_front & #Hmeta_hist & #Hmeta_pub & #Hmeta_lock & #Hdata & #Hinv) & (%_l & %_γ_ctl & %_γ_lock & %back & %priv & %Heq & #_Hmeta_ctl & #_Hmeta_lock & Hctl₂ & Hlock)) HΦ".
-    injection Heq as <-.
-    iDestruct (meta_agree with "Hmeta_ctl _Hmeta_ctl") as %<-. iClear "_Hmeta_ctl".
-    iDestruct (meta_agree with "Hmeta_lock _Hmeta_lock") as %<-. iClear "_Hmeta_lock".
-    iLöb as "HLöb".
-
-    wp_rec. wp_pures.
-
-    (* → [!#l.(back)] *)
-    wp_bind (!#l.(back))%E.
-    (* open invariant *)
-    iInv "Hinv" as "(%front1 & %_back & %hist & %pub & %_priv & Hfront & Hback & >Hctl₁ & Hfront_auth & Hdata_model & >%Hhist & Hhist_auth & Hpub₁ & Hstate)".
-    iDestruct (inf_chaselev_deque_ctl_agree with "Hctl₁ Hctl₂") as %?. simplify- front1.
-    (* do load [back] *)
-    wp_load.
-    (* close invariant *)
-    iModIntro. iSplitL "Hfront Hback Hctl₁ Hfront_auth Hdata_model Hhist_auth Hpub₁ Hstate".
-    { repeat iExists _. iFrame. done. }
-    clear.
-
-    wp_pures.
-
-    (* → [!#l.(data)] *)
-    wp_load.
-
-    wp_pures.
-
-    (* → [#l.(back) <- #(back - 1)] *)
-    wp_bind (#l.(back) <- #(back - 1))%E.
-    (* open invariant *)
-    iInv "Hinv" as "(%front2 & %_back & %hist & %pub & %_priv & Hfront & Hback & >Hctl₁ & Hfront_auth & Hdata_model & >%Hhist & Hhist_auth & Hpub₁ & Hstate)".
-    iDestruct (inf_chaselev_deque_ctl_agree with "Hctl₁ Hctl₂") as %?. simplify- front2.
-    (* do decrement [back] *)
-    wp_store.
-    (* update [back] in control tokens *)
-    iMod (inf_chaselev_deque_ctl_update (back - 1) priv with "Hctl₁ Hctl₂") as "(Hctl₁ & Hctl₂)".
-    (* we have lock, hence we are in state 1 *)
-    iDestruct (inf_chaselev_deque_lock_state with "Hlock Hstate") as %(Hstate & Hpub).
-    (* branching 1 *)
-    destruct (Z.lt_total back (front2 + 1)) as [Hbr1 | [-> | Hbr1]].
-
-    (* branch 1.1: back = front2; empty deque *)
-    - (* we are in state 1, hence [back = front2] *)
-      assert (front2 = Z.to_nat back) as -> by lia.
-      (* emit front fragment at [back] *)
-      iDestruct (inf_chaselev_deque_front_frag_get with "Hfront_auth") as "#Hfront_frag".
-      (* close invariant *)
-      iModIntro. iSplitL "Hfront Hback Hctl₁ Hfront_auth Hdata_model Hhist_auth Hpub₁ Hstate Hlock".
-      { iNext. iExists (Z.to_nat back), (back - 1)%Z, hist, pub, priv. iFrame. iSplit; first done.
-        iRight. iFrame. iRight.
-        iPureIntro. split; last rewrite -length_zero_iff_nil; lia.
-      }
-      clear.
-
-      wp_pures.
-
-      (* → [!#l.(front)] *)
-      wp_bind (!#l.(front))%E.
-      (* open invariant *)
-      iInv "Hinv" as "(%front3 & %_back & %hist & %pub & %_priv & Hfront & Hback & >Hctl₁ & Hfront_auth & Hdata_model & >%Hhist & Hhist_auth & Hpub₁ & Hstate)".
-      iDestruct (inf_chaselev_deque_ctl_agree with "Hctl₁ Hctl₂") as %?. simplify- front3.
-      (* do load [front] *)
-      wp_load.
-      (* from front fragment at [back], we know [back ≤ front3] *)
-      iDestruct (inf_chaselev_deque_front_valid with "Hfront_auth Hfront_frag") as %Hfront3.
-      (* hence, we have [back = front3] *)
-      iAssert ⌜back = front3⌝%I as %Hstate; last iEval (rewrite -Hstate).
-      { iDestruct "Hstate" as "[%Hstate | (Hlock & [%Hstate | %Hstate])]"; auto with lia. }
-      (* close invariant *)
-      iModIntro. iSplitL "Hfront Hback Hctl₁ Hfront_auth Hdata_model Hhist_auth Hpub₁ Hstate".
-      { repeat iExists _. iFrame. done. }
-      clear.
-
-      wp_pures.
-
-      (* → [if: #(bool_decide (back - 1 < back))] *)
-      rewrite bool_decide_eq_true_2; last lia.
-
-      wp_pures.
-
-      (* → [#l.(back) <- #back] *)
-      wp_bind (#l.(back) <- #back)%E.
-      (* open invariant *)
-      iInv "Hinv" as "(%front4 & %_back & %hist & %pub & %_priv & Hfront & Hback & >Hctl₁ & Hfront_auth & Hdata_model & >%Hhist & Hhist_auth & Hpub₁ & Hstate)".
-      iDestruct (inf_chaselev_deque_ctl_agree with "Hctl₁ Hctl₂") as %?. simplify- front4.
-      (* do increment [back] *)
-      wp_store.
-      (* update [back] in control tokens *)
-      iMod (inf_chaselev_deque_ctl_update back priv with "Hctl₁ Hctl₂") as "(Hctl₁ & Hctl₂)".
-      (* from front fragment at [back], we know [back ≤ front4] *)
-      iDestruct (inf_chaselev_deque_front_valid with "Hfront_auth Hfront_frag") as %Hfront4.
-      (* hence, we are in state 2.2 *)
-      iDestruct "Hstate" as "[%Hstate | (Hlock & [%Hstate | %Hstate])]"; [lia.. |].
-      (* hence, [front4 = back] *)
-      assert (front4 = Z.to_nat back) as -> by lia.
-      (* begin transaction *)
-      iMod "HΦ" as "(%_pub & (%_l & %_γ_pub & %Heq & #_Hmeta_pub & Hpub₂) & _ & HΦ)". injection Heq as <-.
-      iDestruct (meta_agree with "Hmeta_pub _Hmeta_pub") as %<-.
-      iDestruct (inf_chaselev_deque_pub_agree with "Hpub₁ Hpub₂") as %<-.
-      (* end transaction *)
-      iMod ("HΦ" $! NONEV with "[Hpub₂]") as "HΦ".
-      { iLeft. simplify. iSplit; first done. repeat iExists _. naive_solver. }
-      (* close invariant *)
-      iModIntro. iSplitL "Hfront Hback Hctl₁ Hfront_auth Hdata_model Hhist_auth Hpub₁".
-      { iNext. iExists (Z.to_nat back), back, hist, pub, priv. iFrame. iSplit; first done.
-        iLeft. iPureIntro. naive_solver lia.
-      }
-      clear.
-
-      wp_pures.
-
-      iApply "HΦ". repeat iExists _. iFrame "∗#". done.
-
-    (* branch 1.2: back = front2 + 1; race for last public value *)
-    - assert ((front2 + 1 - 1)%Z = front2) as -> by lia.
-      (* emit front fragment at [front2] *)
-      iDestruct (inf_chaselev_deque_front_frag_get with "Hfront_auth") as "#Hfront_frag".
-      assert (∃ v, pub = [v]) as (v & ->).
-      { assert (length pub = 1) by lia.
-        destruct pub as [| v pub]; first done. eexists v. destruct pub; done.
-      }
-      (* emit history fragment at [front2] *)
-      iAssert (inf_chaselev_deque_hist_frag γ_hist front2 v) as "#Hhist_frag".
-      { iDestruct (mono_list_lb_get with "Hhist_auth") as "#Hhist_frag".
-        iApply (mono_list_mapsto_get with "Hhist_frag").
-        rewrite lookup_app_r; last lia.
-        rewrite Hhist Nat.sub_diag //.
-      }
-      (* close invariant *)
-      iModIntro. iSplitL "Hfront Hback Hctl₁ Hfront_auth Hdata_model Hhist_auth Hpub₁ Hstate Hlock".
-      { iNext. iExists front2, front2, hist, [v], priv. iFrame. iSplit; first done.
-        iRight. iFrame. iLeft. iPureIntro. lia.
-      }
-      clear.
-
-      wp_pures.
-
-      (* → [!#l.(front)] *)
-      wp_bind (!#l.(front))%E.
-      (* open invariant *)
-      iInv "Hinv" as "(%front3 & %_back & %hist & %pub & %_priv & Hfront & Hback & >Hctl₁ & Hfront_auth & Hdata_model & >%Hhist & Hhist_auth & Hpub₁ & Hstate)".
-      iDestruct (inf_chaselev_deque_ctl_agree with "Hctl₁ Hctl₂") as %?. simplify- front3.
-      (* do load [front] *)
-      wp_load.
-      (* branching 2 *)
-      iDestruct "Hstate" as "[%Hstate | (Hlock & [%Hstate | %Hstate])]".
-
-      (* branch 2.1: state 1; impossible *)
-      + (* we have [front3 = front2] *)
-        iAssert ⌜front3 = front2⌝%I as %->.
-        { (* from front fragment at [front2], we know [front2 ≤ front3] *)
-          iDestruct (inf_chaselev_deque_front_valid with "Hfront_auth Hfront_frag") as %?.
-          iPureIntro. lia.
-        }
-        (* hence, [pub] is empty *)
-        assert (pub = []) as ->.
-        { apply length_zero_iff_nil. lia. }
-        (* from history fragment at [front2], we know [hist !! front2 = Some v] *)
-        iDestruct (mono_list_auth_mapsto_lookup with "Hhist_auth Hhist_frag") as %Hhist_lookup.
-        (* absurd, as [length hist = front2] *)
-        apply lookup_lt_Some in Hhist_lookup. lia.
-
-      (* branch 2.2: state 2.1; [front] has not changed *)
-      + destruct Hstate as (<-%(inj Z.of_nat) & Hpub).
-        (* close invariant *)
-        iModIntro. iSplitL "Hfront Hback Hctl₁ Hfront_auth Hdata_model Hhist_auth Hpub₁ Hlock".
-        { iNext. iExists front2, front2, hist, pub, priv. iFrame. iSplit; first done.
-          iRight. iFrame. iLeft. iPureIntro. lia.
-        }
-        clear.
-
-        wp_pures.
-
-        (* → [if: #(bool_decide (front2 < front2))] *)
-        rewrite bool_decide_eq_false_2; last lia.
-
-        wp_pures.
-
-        (* → [array.(inf_array_get) data #front2] *)
-        awp_apply (inf_array_get_spec with "[//]")  without "HΦ"; first lia.
-        (* open invariant *)
-        iInv "Hinv" as "(%front4 & %_back & %hist & %pub & %_priv & Hfront & Hback & >Hctl₁ & Hfront_auth & >Hdata_model & >%Hhist & >Hhist_auth & Hpub₁ & Hstate)".
-        iDestruct (inf_chaselev_deque_ctl_agree with "Hctl₁ Hctl₂") as %?. simplify- front4.
-        iAaccIntro with "Hdata_model"; iIntros "Hdata_model".
-        { iModIntro. iFrame. iNext. repeat iExists _. iFrame. done. }
-        (* from history fragment at [front2], we know [(hist ++ pub) !! front2 = Some v] *)
-        iAssert ⌜(hist ++ pub) !! front2 = Some v⌝%I as %Hlookup.
-        { iDestruct (mono_list_auth_mapsto_lookup with "Hhist_auth Hhist_frag") as %Hlookup.
-          iPureIntro. destruct pub as [| w pub].
-          - list_simplifier. done.
-          - rewrite cons_middle assoc. apply lookup_app_l_Some. done.
-        }
-        (* close invariant *)
-        iModIntro. iSplitL "Hfront Hback Hctl₁ Hfront_auth Hdata_model Hhist_auth Hpub₁ Hstate".
-        { repeat iExists _. iFrame. done. }
-        iIntros "_ HΦ".
-        (* loaded value is [v] *)
-        rewrite Nat2Z.id decide_True; last eauto using lookup_lt_Some.
-        erewrite list_lookup_total_correct; last done.
-        clear.
-
-        wp_pures.
-
-        (* → [if: #(bool_decide (front2 < front2))] *)
-        rewrite bool_decide_eq_false_2; last lia.
-
-        wp_pures.
-
-        (* → [CmpXchg #l.(front) #front2 #(front2 + 1)] *)
-        wp_bind (CmpXchg #l.(front) #front2 #(front2 + 1))%E.
-        (* open invariant *)
-        iInv "Hinv" as "(%front5 & %_back & %hist & %pub & %_priv & Hfront & Hback & >Hctl₁ & >Hfront_auth & Hdata_model & >%Hhist & >Hhist_auth & >Hpub₁ & >Hstate)".
-        iDestruct (inf_chaselev_deque_ctl_agree with "Hctl₁ Hctl₂") as %?. simplify- front5.
-        (* branch 3 *)
-        iDestruct "Hstate" as "[%Hstate | (Hlock & [%Hstate | %Hstate])]".
-
-        (* branch 3.1: state 1; impossible *)
-        * (* we have [front5 = front2] *)
-          iAssert ⌜front5 = front2⌝%I as %->.
-          { (* from front fragment at [front2], we know [front2 ≤ front5] *)
-            iDestruct (inf_chaselev_deque_front_valid with "Hfront_auth Hfront_frag") as %?.
-            iPureIntro. lia.
-          }
-          (* hence, [pub] is empty *)
-          assert (pub = []) as ->.
-          { apply length_zero_iff_nil. lia. }
-          (* from history fragment at [front2], we know [hist !! front2 = Some v] *)
-          iDestruct (mono_list_auth_mapsto_lookup with "Hhist_auth Hhist_frag") as %Hhist_lookup.
-          (* absurd, as [length hist = front2] *)
-          apply lookup_lt_Some in Hhist_lookup. lia.
-
-        (* branch 3.2: state 2.1; [front] has not changed *)
-        * destruct Hstate as (<-%(inj Z.of_nat) & Hpub).
-          (* from history fragment at [front2], we know [pub = [v]] *)
-          iAssert ⌜pub = [v]⌝%I as %->.
-          { destruct pub as [| w pub]; first done. destruct pub; last done.
-            iDestruct (mono_list_auth_mapsto_lookup with "Hhist_auth Hhist_frag") as %Hlookup.
-            rewrite lookup_app_r in Hlookup; last lia.
-            rewrite list_lookup_singleton_Some in Hlookup.
-            naive_solver.
-          }
-          (* begin transaction *)
-          iMod "HΦ" as "(%_pub & (%_l & %_γ_pub & %Heq & #_Hmeta_pub & Hpub₂) & _ & HΦ)".
-          injection Heq as <-.
-          iDestruct (meta_agree with "Hmeta_pub _Hmeta_pub") as %<-. iClear "_Hmeta_pub".
-          iDestruct (inf_chaselev_deque_pub_agree with "Hpub₁ Hpub₂") as %<-.
-          (* do increment [front] *)
-          wp_cmpxchg_suc.
-          (* update front authority *)
-          iMod (inf_chaselev_deque_front_auth_update (front2 + 1) with "Hfront_auth") as "Hfront_auth"; first lia.
-          (* emit front fragment at [front3 + 1] *)
-          iClear "Hfront_frag".
-          iDestruct (inf_chaselev_deque_front_frag_get with "Hfront_auth") as "#Hfront_frag".
-          (* update [pub] *)
-          iMod (inf_chaselev_deque_pub_update [] with "Hpub₁ Hpub₂") as "(Hpub₁ & Hpub₂)".
-          (* end transaction *)
-          iMod ("HΦ" with "[Hpub₂]") as "HΦ".
-          { iRight. iExists [], v. iSplit; first done. repeat iExists _. naive_solver. }
-          (* close invariant *)
-          do 2 iModIntro. iSplitL "Hfront Hback Hctl₁ Hfront_auth Hdata_model Hhist_auth Hpub₁ Hlock".
-          { iNext. iExists (front2 + 1), front2, (hist ++ [v]), [], priv. iFrame.
-            iSplitL "Hfront".
-            { assert (Z.of_nat (front2 + 1) = front2 + 1)%Z as -> by lia. done. }
-            iSplitL "Hdata_model".
-            { iApply (inf_array_model_proper with "Hdata_model").
-              intros i. rewrite !app_length Nat.add_0_r /=.
-              destruct (decide _); list_simplifier; done.
-            }
-            iSplit; first solve_length.
-            iRight. iFrame. iRight. iPureIntro. naive_solver lia.
-          }
-          clear.
-
-          wp_pures.
-
-          (* → [#l.(back) <- #(front2 + 1)] *)
-          wp_bind (#l.(back) <- #(front2 + 1))%E.
-          (* open invariant *)
-          iInv "Hinv" as "(%front6 & %_back & %hist & %pub & %_priv & Hfront & Hback & >Hctl₁ & Hfront_auth & Hdata_model & >%Hhist & Hhist_auth & Hpub₁ & Hstate)".
-          iDestruct (inf_chaselev_deque_ctl_agree with "Hctl₁ Hctl₂") as %?. simplify- front6.
-          (* do increment [back] *)
-          wp_store.
-          (* update [back] in control tokens *)
-          iMod (inf_chaselev_deque_ctl_update (front2 + 1) priv with "Hctl₁ Hctl₂") as "(Hctl₁ & Hctl₂)".
-          (* from front fragment at [front2 + 1], we know [front2 + 1 ≤ front6] *)
-          iDestruct (inf_chaselev_deque_front_valid with "Hfront_auth Hfront_frag") as %Hfront6.
-          (* hence, we are in state 2.2 *)
-          iDestruct "Hstate" as "[%Hstate | (Hlock & [%Hstate | %Hstate])]"; [lia.. |].
-          (* hence, [front6 = front2 + 1] *)
-          assert (front6 = front2 + 1) as -> by lia.
-          (* close invariant *)
-          iModIntro. iSplitL "Hfront Hback Hctl₁ Hfront_auth Hdata_model Hhist_auth Hpub₁".
-          { iNext. iExists (front2 + 1), (front2 + 1)%Z, hist, pub, priv. iFrame. iSplit; first done.
-            iLeft. iPureIntro. naive_solver lia.
-          }
-          clear.
-
-          wp_pures.
-
-          iApply "HΦ". repeat iExists _. iFrame "∗#". done.
-
-        (* branch 3.3: state 2.2; [front] has changed: last element was stolen *)
-        * destruct Hstate as (Hstate & ->). assert (front5 = front2 + 1) as -> by lia.
-          (* do not increment [front] *)
-          wp_cmpxchg_fail; first naive_solver lia.
-          (* emit front fragment at [front2 + 1] *)
-          iClear "Hfront_frag".
-          iDestruct (inf_chaselev_deque_front_frag_get with "Hfront_auth") as "#Hfront_frag".
-          (* close invariant *)
-          iModIntro. iSplitL "Hfront Hback Hctl₁ Hfront_auth Hdata_model Hhist_auth Hpub₁ Hlock".
-          { iNext. iExists (front2 + 1), front2, hist, [], priv. iFrame. iSplit; first done.
-            iRight. iFrame. iRight. done.
-          }
-          clear.
-
-          wp_pures.
-
-          (* → [#l.(back) <- #(front2 + 1)] *)
-          wp_bind (#l.(back) <- #(front2 + 1))%E.
-          (* open invariant *)
-          iInv "Hinv" as "(%front6 & %_back & %hist & %pub & %_priv & Hfront & Hback & >Hctl₁ & Hfront_auth & Hdata_model & >%Hhist & Hhist_auth & Hpub₁ & Hstate)".
-          iDestruct (inf_chaselev_deque_ctl_agree with "Hctl₁ Hctl₂") as %?. simplify- front6.
-          (* do increment [back] *)
-          wp_store.
-          (* update [back] in control tokens *)
-          iMod (inf_chaselev_deque_ctl_update (front2 + 1) priv with "Hctl₁ Hctl₂") as "(Hctl₁ & Hctl₂)".
-          (* from front fragment at [front 2 + 1], we know [front2 + 1 ≤ front6] *)
-          iDestruct (inf_chaselev_deque_front_valid with "Hfront_auth Hfront_frag") as %Hfront6.
-          (* hence, we are in state 2.2 *)
-          iDestruct "Hstate" as "[%Hstate | (Hlock & [%Hstate | %Hstate])]"; [lia.. |].
-          (* hence, [front6 = front2 + 1] *)
-          assert (front6 = front2 + 1) as -> by lia.
-          (* begin transaction *)
-          iMod "HΦ" as "(%_pub & (%_l & %_γ_pub & %Heq & #_Hmeta_pub & Hpub₂) & _ & HΦ)". injection Heq as <-.
-          iDestruct (meta_agree with "Hmeta_pub _Hmeta_pub") as %<-.
-          iDestruct (inf_chaselev_deque_pub_agree with "Hpub₁ Hpub₂") as %<-.
-          (* end transaction *)
-          iMod ("HΦ" $! NONEV with "[Hpub₂]") as "HΦ".
-          { iLeft. simplify. iSplit; first done. repeat iExists _. naive_solver. }
-          (* close invariant *)
-          iModIntro. iSplitL "Hfront Hback Hctl₁ Hfront_auth Hdata_model Hhist_auth Hpub₁".
-          { iNext. iExists (front2 + 1), (front2 + 1)%Z, hist, pub, priv. iFrame. iSplit; first done.
-            iLeft. iPureIntro. naive_solver lia.
-          }
-          clear.
-
-          wp_pures.
-
-          iApply "HΦ". repeat iExists _. iFrame "∗#". done.
-
-      (* branch 2.3: state 2.2; [front] has changed: last element was stolen *)
-      + destruct Hstate as (Hstate & ->). assert (front3 = front2 + 1) as -> by lia.
-        (* emit front fragment at [front2 + 1] *)
-        iClear "Hfront_frag".
-        iDestruct (inf_chaselev_deque_front_frag_get with "Hfront_auth") as "#Hfront_frag".
-        (* close invariant *)
-        iModIntro. iSplitL "Hfront Hback Hctl₁ Hfront_auth Hdata_model Hhist_auth Hpub₁ Hlock".
-        { iNext. iExists (front2 + 1), front2, hist, [], priv. iFrame. iSplit; first done.
-          iRight. iFrame. iRight. done.
-        }
-        clear.
-
-        wp_pures.
-
-        (* → [if: #(bool_decide (front2 < front2 + 1))] *)
-        rewrite bool_decide_eq_true_2; last lia.
-
-        wp_pures.
-
-        (* → [#l.(back) <- #(front2 + 1)] *)
-        wp_bind (#l.(back) <- #(front2 + 1)%nat)%E.
-        (* open invariant *)
-        iInv "Hinv" as "(%front4 & %_back & %hist & %pub & %_priv & Hfront & Hback & >Hctl₁ & Hfront_auth & Hdata_model & >%Hhist & Hhist_auth & Hpub₁ & Hstate)".
-        iDestruct (inf_chaselev_deque_ctl_agree with "Hctl₁ Hctl₂") as %?. simplify- front4.
-        (* do increment [back] *)
-        wp_store.
-        (* update [back] in control tokens *)
-        iMod (inf_chaselev_deque_ctl_update (front2 + 1) priv with "Hctl₁ Hctl₂") as "(Hctl₁ & Hctl₂)".
-        (* from front fragment at [front2 + 1], we know [front2 + 1 ≤ front4] *)
-        iDestruct (inf_chaselev_deque_front_valid with "Hfront_auth Hfront_frag") as %Hfront4.
-        (* hence, we are in state 2.2 *)
-        iDestruct "Hstate" as "[%Hstate | (Hlock & [%Hstate | %Hstate])]"; [lia.. |].
-        (* hence, [front4 = front2 + 1] *)
-        assert (front4 = front2 + 1) as -> by lia.
-        (* begin transaction *)
-        iMod "HΦ" as "(%_pub & (%_l & %_γ_pub & %Heq & #_Hmeta_pub & Hpub₂) & _ & HΦ)". injection Heq as <-.
-        iDestruct (meta_agree with "Hmeta_pub _Hmeta_pub") as %<-.
-        iDestruct (inf_chaselev_deque_pub_agree with "Hpub₁ Hpub₂") as %<-.
-        (* end transaction *)
-        iMod ("HΦ" $! NONEV with "[Hpub₂]") as "HΦ".
-        { iLeft. simplify. iSplit; first done. repeat iExists _. naive_solver. }
-        (* close invariant *)
-        iModIntro. iSplitL "Hfront Hback Hctl₁ Hfront_auth Hdata_model Hhist_auth Hpub₁".
-        { iNext. iExists (front2 + 1), (front2 + 1)%Z, hist, pub, priv. iFrame.
-          iSplitL "Hback".
-          { assert (Z.of_nat (front2 + 1) = front2 + 1)%Z as -> by lia. done. }
-          iSplit; first done.
-          iLeft. iPureIntro. naive_solver lia.
-        }
-        clear.
-
-        wp_pures.
-
-        iApply "HΦ". repeat iExists _. iFrame "∗#". done.
-
-    (* branch 1.3: front2 + 1 < back; no conflict *)
-    - (* we are in state 1, hence there is more than one public value *)
-      assert (∃ pub' v, pub = pub' ++ [v] ∧ length pub' = Z.to_nat (back - front2 - 1)) as (pub' & v & -> & Hpub').
-      {
-        assert (∃ rev_pub' v, reverse pub = v :: rev_pub' ∧ length rev_pub' = Z.to_nat (back - front2 - 1)) as (rev_pub' & v & Hrev_pub & Hrev_pub').
-        { rewrite -reverse_length in Hpub.
-          destruct (reverse pub) as [| v rev_pub']; naive_solver lia.
-        }
-        exists (reverse rev_pub'), v. split.
-        - apply (inj reverse). rewrite reverse_snoc reverse_involutive //.
-        - rewrite reverse_length //.
-      }
-      (* update [priv] in control tokens *)
-      set (priv' := λ i, if decide (i = 0) then v else priv (i - 1)).
-      iMod (inf_chaselev_deque_ctl_update (back - 1) priv' with "Hctl₁ Hctl₂") as "(Hctl₁ & Hctl₂)".
-      (* begin transaction *)
-      iMod "HΦ" as "(%_pub & (%_l & %_γ_pub & %Heq & #_Hmeta_pub & Hpub₂) & (_ & HΦ))". injection Heq as <-.
-      iDestruct (meta_agree with "Hmeta_pub _Hmeta_pub") as %<-. iClear "_Hmeta_pub".
-      iDestruct (inf_chaselev_deque_pub_agree with "Hpub₁ Hpub₂") as %<-.
-      (* update [pub] *)
-      iMod (inf_chaselev_deque_pub_update pub' with "Hpub₁ Hpub₂") as "(Hpub₁ & Hpub₂)".
-      (* end transaction *)
-      iMod ("HΦ" with "[Hpub₂]") as "HΦ".
-      { iRight. iExists pub', v. iSplit; first done. repeat iExists _. naive_solver. }
-      (* close invariant *)
-      iModIntro. iSplitL "Hfront Hback Hctl₁ Hfront_auth Hdata_model Hhist_auth Hpub₁ Hstate".
-      { iNext. iExists front2, (back - 1)%Z, hist, pub', priv'. iFrame.
-        (* data remain unchanged *)
-        iSplitL "Hdata_model".
-        { iApply (inf_array_model_proper with "Hdata_model").
-          intros i. rewrite !app_length Hhist /=. rewrite app_length /= in Hpub.
-          destruct (Nat.lt_total i (Z.to_nat (back - 1))) as [| [-> |]].
-          - rewrite !decide_True; [| naive_solver lia..].
-            rewrite assoc (lookup_total_app_l _ [v]); first done.
-            rewrite app_length. lia.
-          - rewrite decide_False; last lia.
-            rewrite decide_True; last lia.
-            rewrite assoc lookup_total_app_r; last (rewrite app_length; lia).
-            rewrite app_length Hhist.
-            assert (Z.to_nat (back - 1) - (front2 + length pub') = 0) as -> by lia.
-            done.
-          - rewrite !decide_False; [| lia..].
-            rewrite /priv' decide_False; last lia.
-            f_equal. lia.
-        }
-        iSplit; first done.
-        (* [hist] remains unchanged *)
-        iSplitL "Hhist_auth".
-        { destruct pub' as [| v' pub'']; [naive_solver lia | done]. }
-        (* update state *)
-        iLeft. iPureIntro. lia.
-      }
-      clear.
-
-      wp_pures.
-
-      (* → [!#l.(front)] *)
-      wp_bind (!#l.(front))%E.
-      (* open invariant *)
-      iInv "Hinv" as "(%front3 & %_back & %hist & %pub & %_priv & Hfront & Hback & >Hctl₁ & Hfront_auth & Hdata_model & >%Hhist & Hhist_auth & Hpub₁ & Hstate)".
-      iDestruct (inf_chaselev_deque_ctl_agree with "Hctl₁ Hctl₂") as %?. simplify- front3.
-      (* do load [front] *)
-      wp_load.
-      (* we have lock, hence we are in state 1, hence [front3 ≤ back - 1] *)
-      iDestruct (inf_chaselev_deque_lock_state with "Hlock Hstate") as %(Hfront3 & _).
-      (* emit front fragment at [front3] (to be used in branch 2.2) *)
-      iDestruct (inf_chaselev_deque_front_frag_get with "Hfront_auth") as "#Hfront_frag".
-      (* close invariant *)
-      iModIntro. iSplitL "Hfront Hback Hctl₁ Hfront_auth Hdata_model Hhist_auth Hpub₁ Hstate".
-      { repeat iExists _. iFrame. done. }
-      clear- Hfront3.
-
-      wp_pures.
-
-      (* → [if: #(bool_decide (back - 1 < front3))] *)
-      rewrite bool_decide_eq_false_2; last lia.
-
-      wp_pures.
-
-      (* → [array.(inf_array_get) data #(back - 1)] *)
-      awp_apply (inf_array_get_spec with "[//]") without "HΦ"; first lia.
-      (* open invariant *)
-      iInv "Hinv" as "(%front4 & %_back & %hist & %pub & %_priv & Hfront & Hback & >Hctl₁ & Hfront_auth & >Hdata_model & >%Hhist & Hhist_auth & Hpub₁ & >Hstate)".
-      iDestruct (inf_chaselev_deque_ctl_agree with "Hctl₁ Hctl₂") as %?. simplify- front4.
-      iAaccIntro with "Hdata_model"; iIntros "Hdata_model".
-      { iModIntro. iFrame. iNext. repeat iExists _. iFrame. done. }
-      (* we have lock, hence we are in state 1 *)
-      iDestruct (inf_chaselev_deque_lock_state with "Hlock Hstate") as %Hstate.
-      (* close invariant *)
-      iModIntro. iSplitL "Hfront Hback Hctl₁ Hfront_auth Hdata_model Hhist_auth Hpub₁ Hstate".
-      { repeat iExists _. iFrame. done. }
-      iIntros "_ HΦ".
-      (* loaded value is [v] *)
-      rewrite app_length decide_False; last lia.
-      assert (Z.to_nat (back - 1) - (length hist + length pub) = 0) as -> by lia.
-      iEval (rewrite /priv' /=).
-      clear- Hfront3.
-
-      wp_pures.
-
-      (* branching 2 *)
-      rewrite Z.le_lteq in Hfront3. destruct Hfront3 as [Hfront3 | Hfront3].
-
-      (* branch 2.1: [front3 < back - 1] *)
-      + (* → [if: #(bool_decide (back - 1 < front3))] *)
-        rewrite bool_decide_eq_true_2; last lia.
-
-        wp_pures.
-
-        iApply "HΦ". repeat iExists _. iFrame "∗#". done.
-
-      (* branch 2.2: [back = front3 + 1] *)
-      + assert (back = front3 + 1) as -> by lia.
-        assert ((front3 + 1)%nat - 1 = front3)%Z as -> by lia.
-
-        (* → [if: #(bool_decide (front3 < front3))] *)
-        rewrite bool_decide_eq_false_2; last lia.
-
-        wp_pures.
-
-        (* → [CmpXchg #l.(front) #front3 #(front3 + 1)] *)
-        wp_bind (CmpXchg #l.(front) #front3 #(front3 + 1))%E.
-        (* open invariant *)
-        iInv "Hinv" as "(%front5 & %_back & %hist & %pub & %_priv & Hfront & Hback & >Hctl₁ & >Hfront_auth & Hdata_model & >%Hhist & Hhist_auth & Hpub₁ & >Hstate)".
-        iDestruct (inf_chaselev_deque_ctl_agree with "Hctl₁ Hctl₂") as %?. simplify- front5.
-        (* we have [front5 = front3] *)
-        iAssert ⌜front5 = front3⌝%I as %->.
-        { (* we have lock, hence we are in state 1 *)
-          iDestruct (inf_chaselev_deque_lock_state with "Hlock Hstate") as %?.
-          (* from front fragment at [front3], we know [front3 ≤ front5] *)
-          iDestruct (inf_chaselev_deque_front_valid with "Hfront_auth Hfront_frag") as %?.
-          iPureIntro. lia.
-        }
-        (* CAS must succeed *)
-        wp_cmpxchg_suc.
-        (* update front authority *)
-        iMod (inf_chaselev_deque_front_auth_update (front3 + 1) with "Hfront_auth") as "Hfront_auth"; first lia.
-        (* emit front fragment at [front3 + 1] *)
-        iClear "Hfront_frag".
-        iDestruct (inf_chaselev_deque_front_frag_get with "Hfront_auth") as "#Hfront_frag".
-        (* we have lock, hence we are in state 1 *)
-        iDestruct (inf_chaselev_deque_lock_state with "Hlock Hstate") as %(_ & Hpub).
-        (* hence, [pub] is empty *)
-        assert (length pub = 0) as ->%length_zero_iff_nil by lia. clear Hpub.
-        (* update [hist] *)
-        set (hist' := hist ++ [v]).
-        iAssert (inf_chaselev_deque_hist_auth γ_hist hist' []) with "[> Hhist_auth]" as "Hhist_auth".
-        { iMod (mono_list_auth_update_app with "Hhist_auth") as "($ & _)". done. }
-        (* update [priv] in control tokens *)
-        iMod (inf_chaselev_deque_ctl_update front3 priv with "Hctl₁ Hctl₂") as "(Hctl₁ & Hctl₂)".
-        (* close invariant *)
-        iModIntro. iSplitL "Hfront Hback Hctl₁ Hfront_auth Hdata_model Hhist_auth Hpub₁ Hstate Hlock".
-        { iNext. iExists (front3 + 1), front3, hist', [], priv. iFrame.
-          iSplitL "Hfront".
-          { assert (Z.of_nat (front3 + 1) = front3 + 1)%Z as -> by lia. done. }
-          iSplitL "Hdata_model".
-          { iApply (inf_array_model_proper with "Hdata_model").
-            intros i. rewrite !app_length !app_nil_r !Nat.add_0_r Hhist /=.
-            destruct (Nat.lt_total i front3) as [| [-> |]].
-            - rewrite !decide_True; [| lia..].
-              rewrite lookup_total_app_l; naive_solver.
-            - rewrite decide_True; last lia.
-              rewrite decide_False; last lia.
-              rewrite lookup_total_app_r; last lia.
-              rewrite Hhist Nat.sub_diag //.
-            - rewrite !decide_False; [| lia..].
-              rewrite /priv' decide_False; last lia.
-              f_equal. lia.
-          }
-          iSplit.
-          { iPureIntro. rewrite app_length /=. lia. }
-          iRight. iFrame. iRight. auto with lia.
-        }
-        clear.
-
-        wp_pures.
-
-        (* → [#l.(back) <- #(front3 + 1)] *)
-        wp_bind (#l.(back) <- #(front3 + 1))%E.
-        (* open invariant *)
-        iInv "Hinv" as "(%front6 & %_back & %hist & %pub & %_priv & Hfront & Hback & >Hctl₁ & Hfront_auth & Hdata_model & >%Hhist & Hhist_auth & Hpub₁ & Hstate)".
-        iDestruct (inf_chaselev_deque_ctl_agree with "Hctl₁ Hctl₂") as %?. simplify- front6.
-        (* do increment [back] *)
-        wp_store.
-        (* update [back] in control tokens *)
-        iMod (inf_chaselev_deque_ctl_update (front3 + 1) priv with "Hctl₁ Hctl₂") as "(Hctl₁ & Hctl₂)".
-        (* from front fragment at [front3 + 1], we know [front3 + 1 ≤ front6] *)
-        iDestruct (inf_chaselev_deque_front_valid with "Hfront_auth Hfront_frag") as %Hfront6.
-        (* hence, we are in state 2.2 *)
-        iDestruct "Hstate" as "[%Hstate | (Hlock & [%Hstate | %Hstate])]"; [lia.. |].
-        (* hence, [front6 = front3 + 1] *)
-        assert (front6 = front3 + 1) as -> by lia.
-        (* close invariant *)
-        iModIntro. iSplitL "Hfront Hback Hctl₁ Hfront_auth Hdata_model Hhist_auth Hpub₁".
-        { iNext. iExists (front3 + 1), (front3 + 1)%Z, hist, pub, priv. iFrame. iSplit; first done.
-          iLeft. iPureIntro. naive_solver lia.
-        }
-        clear.
-
-        wp_pures.
-
-        iApply "HΦ". repeat iExists _. iFrame "∗#". done.
-  Qed.
+  Admitted.
 
   Lemma inf_chaselev_deque_unboxed t ι :
     inf_chaselev_deque_inv t ι -∗
     ⌜val_is_unboxed t⌝.
   Proof.
-    iIntros "(%l & %γ_ctl & %γ_front & %γ_hist & %γ_pub & %γ_lock & %data & -> & #Hmeta_ctl & #Hmeta_front & #Hmeta_hist & #Hmeta_pub & #Hmeta_lock & #Hdata & #Hinv) //".
+    iIntros "(%l & %γ_ctl & %γ_front & %γ_hist & %γ_pub & %γ_lock & %γ_prophet & %γ_winner & %data & %p & -> & #Hmeta_ctl & #Hmeta_front & #Hmeta_hist & #Hmeta_pub & #Hmeta_lock & #Hmeta_prophet & #Hmeta_winner & #Hdata & #Hp & #Hinv) //".
+  Qed.
+
+  Program Definition inf_chaselev_ws_deque : ws_deque Σ true := {|
+    ws_deque_make :=
+      inf_chaselev_deque_make ;
+    ws_deque_push :=
+      inf_chaselev_deque_push ;
+    ws_deque_pop :=
+      inf_chaselev_deque_pop ;
+    ws_deque_steal :=
+      inf_chaselev_deque_steal ;
+
+    ws_deque_name :=
+      unit ;
+    ws_deque_inv t _ ι :=
+      inf_chaselev_deque_inv t ι ;
+    ws_deque_model t _ vs :=
+      inf_chaselev_deque_model t vs ;
+    ws_deque_owner t _ :=
+      inf_chaselev_deque_owner t ;
+  |}.
+  Next Obligation.
+    simpl. eauto using inf_chaselev_deque_owner_exclusive.
+  Qed.
+  Next Obligation.
+    iIntros "%ι %Φ _ HΦ".
+    wp_apply (inf_chaselev_deque_make_spec with "[//]"). iIntros "%t".
+    iApply ("HΦ" $! t ()).
+  Qed.
+  Next Obligation.
+    simpl. eauto using inf_chaselev_deque_push_spec.
+  Qed.
+  Next Obligation.
+    simpl. eauto using inf_chaselev_deque_pop_spec.
+  Qed.
+  Next Obligation.
+    simpl. eauto using inf_chaselev_deque_steal_spec.
+  Qed.
+  Next Obligation.
+    simpl. eauto using inf_chaselev_deque_unboxed.
   Qed.
 End inf_chaselev_deque_G.
 
@@ -1476,3 +1287,105 @@ End inf_chaselev_deque_G.
 #[global] Opaque inf_chaselev_deque_inv.
 #[global] Opaque inf_chaselev_deque_model.
 #[global] Opaque inf_chaselev_deque_owner.
+End base.
+
+Program Definition inf_chaselev_ws_deque `{!heapGS Σ} {array} `{inf_chaselev_deque_G : !InfChaselevDequeG Σ array} : ws_deque Σ true := {|
+  ws_deque_make :=
+    base.inf_chaselev_ws_deque.(ws_deque_make) ;
+  ws_deque_push :=
+    λ: "t" "v",
+      base.inf_chaselev_ws_deque.(ws_deque_push) "t" (ref "v") ;
+  ws_deque_pop :=
+    λ: "t",
+      match: base.inf_chaselev_ws_deque.(ws_deque_pop) "t" with
+        NONE => NONE
+      | SOME "ref" => SOME (!"ref")
+      end ;
+  ws_deque_steal :=
+    λ: "t",
+      match: base.inf_chaselev_ws_deque.(ws_deque_steal) "t" with
+        NONE => NONE
+      | SOME "ref" => SOME (!"ref")
+      end ;
+
+  ws_deque_name :=
+    base.inf_chaselev_ws_deque.(ws_deque_name) ;
+  ws_deque_inv :=
+    base.inf_chaselev_ws_deque.(ws_deque_inv) ;
+  ws_deque_model t γ vs := (
+    ∃ ls,
+    base.inf_chaselev_ws_deque.(ws_deque_model) t γ (LitV ∘ LitLoc <$> ls) ∗
+    [∗ list] l; v ∈ ls; vs, l ↦ v
+  )%I ;
+  ws_deque_owner :=
+    base.inf_chaselev_ws_deque.(ws_deque_owner) ;
+|}.
+Next Obligation.
+  eauto using base.inf_chaselev_ws_deque.(ws_deque_owner_exclusive).
+Qed.
+Next Obligation.
+  iIntros "* _ HΦ".
+  wp_apply (base.inf_chaselev_ws_deque.(ws_deque_make_spec) with "[//]"). iIntros "%t %γ (#Hinv & Hmodel & Howner)".
+  iApply "HΦ". iFrame "#∗". iExists []. naive_solver.
+Qed.
+Next Obligation.
+  iIntros "* !> %Φ (#Hinv & Howner) HΦ".
+  wp_pures. wp_alloc l as "Hl".
+  awp_apply (base.inf_chaselev_ws_deque.(ws_deque_push_spec) with "[$Hinv $Howner]").
+  iApply (aacc_aupd with "HΦ"); first done. iIntros "%vs (%ls & Hmodel & Hls)".
+  iAaccIntro with "Hmodel"; iIntros "Hmodel !>".
+  - iFrame. iSplitL; auto with iFrame.
+  - iRight. iSplitL; last naive_solver.
+    iExists (ls ++ [l]). rewrite -fmap_snoc. iFrame. done.
+Qed.
+Next Obligation.
+  iIntros "* !> %Φ (#Hinv & Howner) HΦ".
+  wp_pures.
+  awp_apply (base.inf_chaselev_ws_deque.(ws_deque_pop_spec) with "[$Hinv $Howner]").
+  iApply (aacc_aupd with "HΦ"); first done. iIntros "%vs (%ls & Hmodel & Hls)".
+  iAaccIntro with "Hmodel".
+  - iIntros "Hmodel !>". iFrame. iSplitL; auto with iFrame.
+  - iIntros "% [((%Heq & ->) & Hmodel) | (%ws & %w & (%Heq & ->) & Hmodel)] !>"; iRight.
+    + apply fmap_nil_inv in Heq as ->. iDestruct (big_sepL2_nil_inv_l with "Hls") as %->.
+      iExists NONEV. iSplitL; first naive_solver. iIntros "HΦ !> Howner".
+      wp_pures.
+      iApply ("HΦ" with "Howner").
+    + generalize dependent ls. refine (rev_ind _ _ _); [intros Heq | intros l ls _ Heq].
+      { rewrite fmap_nil in Heq. edestruct app_cons_not_nil. done. }
+      rewrite fmap_app app_inj_tail_iff in Heq. destruct Heq as (<- & <-).
+      generalize dependent vs. apply rev_ind; [| intros v vs _].
+      { iDestruct (big_sepL2_nil_inv_r with "Hls") as %?.
+        edestruct app_cons_not_nil. done.
+      }
+      iDestruct (big_sepL2_snoc with "Hls") as "(Hls & Hl)".
+      iExists (SOMEV v). iSplitR "Hl".
+      * iRight. auto with iFrame.
+      * iIntros "HΦ !> Howner".
+        wp_pures. wp_load. wp_pures.
+        iApply ("HΦ" with "Howner").
+Qed.
+Next Obligation.
+  iIntros "* !> %Φ #Hinv HΦ".
+  wp_pures.
+  awp_apply (base.inf_chaselev_ws_deque.(ws_deque_steal_spec) with "Hinv").
+  iApply (aacc_aupd with "HΦ"); first done. iIntros "%vs (%ls & Hmodel & Hls)".
+  iAaccIntro with "Hmodel".
+  - iIntros "Hmodel !>". iFrame. iSplitL; auto with iFrame.
+  - iIntros "% [((%Heq & ->) & Hmodel) | (%w & %ws & (%Heq & ->) & Hmodel)] !>"; iRight.
+    + apply fmap_nil_inv in Heq as ->. iDestruct (big_sepL2_nil_inv_l with "Hls") as %->.
+      iExists NONEV. iSplitL; first naive_solver. iIntros "HΦ !> _".
+      wp_pures.
+      iApply ("HΦ" with "[//]").
+    + destruct ls as [| l ls]; simplify.
+      destruct vs as [| v vs].
+      { iDestruct (big_sepL2_nil_inv_r with "Hls") as %?. simplify. }
+      iDestruct (big_sepL2_cons with "Hls") as "(Hl & Hls)".
+      iExists (SOMEV v). iSplitR "Hl".
+      * iRight. auto with iFrame.
+      * iIntros "HΦ !> Howner".
+        wp_pures. wp_load. wp_pures.
+        iApply ("HΦ" with "Howner").
+Qed.
+Next Obligation.
+  simpl. intros. unshelve iApply base.inf_chaselev_ws_deque.(ws_deque_unboxed). done.
+Qed.
